Grzegorczyk Logic (Grz) via modal translation

make.ml
@@ -12,49 +12,69 @@
 (* Libraries.                                                                *)
 (* ------------------------------------------------------------------------- *)
 
-needs "Library/card.ml";;                (* Cardinality                      *)
-needs "Library/rstc.ml";;                (* Refl, sym, trans closure         *)
+needs "Library/card.ml";;                    (* Cardinality                 *)
+needs "Library/rstc.ml";;                    (* Refl, sym, trans closure    *)
 
 (* ------------------------------------------------------------------------- *)
 (* Syntax, semantics and calculus.                                           *)
 (* ------------------------------------------------------------------------- *)
 
-loadt "HOLMS/misc.ml";;                (* Miscellanea                        *)
-loadt "HOLMS/modal.ml";;               (* Syntax and semantics               *)
-loadt "HOLMS/calculus.ml";;            (* Axiomatic calculus                 *)
+loadt "HOLMS/misc.ml";;                      (* Miscellanea                 *)
+loadt "HOLMS/modal.ml";;                     (* Syntax and semantics        *)
+loadt "HOLMS/calculus.ml";;                  (* Axiomatic calculus          *)
 
 (* ------------------------------------------------------------------------- *)
 (* Correspondence Theory.                                                    *)
 (* ------------------------------------------------------------------------- *)
 
-loadt "HOLMS/ad_hoc_correspondence.ml";;       (* Ad hoc polimorphic code    *)
 loadt "HOLMS/parametric_correspondence.ml";;   (* Parametric code            *)
+loadt "HOLMS/ad_hoc_correspondence.ml";;       (* Ad hoc polimorphic code    *)
 
 (* ------------------------------------------------------------------------- *)
 (* Meta-theory.                                                              *)
 (* ------------------------------------------------------------------------- *)
 
-loadt "HOLMS/conjlist.ml";;            (* Iterated conjunctions              *)
-loadt "HOLMS/consistent.ml";;          (* Consistent sets of formulae        *)
-loadt "HOLMS/gen_completeness.ml";;    (* Lemmata about completeness         *)
-loadt "HOLMS/k_completeness.ml";;      (* Completeness of K                  *)
-loadt "HOLMS/t_completeness.ml";;      (* Completeness of T                  *)
-loadt "HOLMS/k4_completeness.ml";;     (* Completeness of K4                 *)
-loadt "HOLMS/s4_completeness.ml";;     (* Completeness of S4                 *)
-loadt "HOLMS/b_completeness.ml";;      (* Completeness of B                  *)
-loadt "HOLMS/s5_completeness.ml";;     (* Completeness of S5                 *)
-loadt "HOLMS/gl_completeness.ml";;     (* Completeness of GL                 *)
+loadt "HOLMS/conjlist.ml";;                  (* Iterated conjunctions       *)
+loadt "HOLMS/consistent.ml";;                (* Consistent sets of formulae *)
+loadt "HOLMS/gen_completeness.ml";;          (* Lemmata about completeness  *)
 
 (* ------------------------------------------------------------------------- *)
-(* Decision procedures.                                                      *)
+(* Soundness and completeness results specific to each logic.                *)
 (* ------------------------------------------------------------------------- *)
 
-loadt "HOLMS/gen_decid.ml";;           (* Tools for decidability             *)
-loadt "HOLMS/gen_countermodel.ml";;    (* Tools for countermodels            *)
-loadt "HOLMS/k_decid.ml";;             (* Semidecision procedure for K       *)
-loadt "HOLMS/t_decid.ml";;             (* Semidecision procedure for T       *)
-loadt "HOLMS/k4_decid.ml";;            (* Semidecision procedure for K4      *)
-loadt "HOLMS/s4_decid.ml";;            (* Semidecision procedure for S4      *)
-loadt "HOLMS/b_decid.ml";;             (* Semidecision procedure for B       *)
-loadt "HOLMS/s5_decid.ml";;            (* Semidecision procedure for S5      *)
-loadt "HOLMS/gl_decid.ml";;            (* Semidecision procedure for GL      *)
+loadt "HOLMS/k_completeness.ml";;
+loadt "HOLMS/t_completeness.ml";;
+loadt "HOLMS/k4_completeness.ml";;
+loadt "HOLMS/s4_completeness.ml";;
+loadt "HOLMS/b_completeness.ml";;
+loadt "HOLMS/s5_completeness.ml";;
+loadt "HOLMS/gl_completeness.ml";;
+
+(* ------------------------------------------------------------------------- *)
+(* General tools for decidability and countermodel generation.               *)
+(* ------------------------------------------------------------------------- *)
+
+loadt "HOLMS/gen_decid.ml";;
+loadt "HOLMS/gen_countermodel.ml";;
+
+(* ------------------------------------------------------------------------- *)
+(* Decision procedures and countermodel generators specific to each logic.   *)
+(* ------------------------------------------------------------------------- *)
+
+loadt "HOLMS/k_decid.ml";;
+loadt "HOLMS/t_decid.ml";;
+loadt "HOLMS/k4_decid.ml";;
+loadt "HOLMS/s4_decid.ml";;
+loadt "HOLMS/b_decid.ml";;
+loadt "HOLMS/s5_decid.ml";;
+loadt "HOLMS/gl_decid.ml";;
+
+(* ------------------------------------------------------------------------- *)
+(* Grzegorczyk Logic (GRZ): Meta-theory, translations to GL,                 *)
+(* decision procedure (via translation to GL).                               *)
+(* ------------------------------------------------------------------------- *)
+
+loadt "HOLMS/translations.ml";;
+loadt "HOLMS/grz.ml";;
+loadt "HOLMS/grz_tests.ml";;
+loadt "HOLMS/god_transl.ml";;
