translations.ml
@@ -6,26 +6,6 @@
 (* ========================================================================= *)
 
 (* ------------------------------------------------------------------------- *)
-(* Run a conversion.                                                         *)
-(* ------------------------------------------------------------------------- *)
-
-let run_conv (conv:conv) tm =
-  let etm =
-    try concl (conv tm)
-    with Failure _ -> failwith "run_conv: Conversion fails" in
-  try rhs etm
-  with Failure _ -> failwith "run_conv: Not equational";;  
-
-(* ------------------------------------------------------------------------- *)
-(* Check the result of a conversion.                                         *)
-(* ------------------------------------------------------------------------- *)
-
-let check_conv conv tm1 tm2 =
-  let tm = try run_conv conv tm1
-           with Failure s -> failwith ("check_conv: "^s) in
-  if tm = tm2 then () else failwith "check_conv: Not the expected result";; 
-
-(* ------------------------------------------------------------------------- *)
 (* Translation: Box  ~~>  Dotbox.                                            *)
 (* ------------------------------------------------------------------------- *)
 
@@ -46,15 +26,15 @@ let TRANSL_CONV:conv = REWRITE_CONV[TRANSL];;
 (* Tests.                                                                    *)
 (* ------------------------------------------------------------------------- *)
 
-check_conv TRANSL_CONV `TRANSL (Atom a)` `Atom a`;;
-check_conv TRANSL_CONV `TRANSL True` `True`;;
-check_conv TRANSL_CONV `TRANSL False` `False`;;
-check_conv TRANSL_CONV `TRANSL (Not True)` `Not True`;;
-check_conv TRANSL_CONV `TRANSL (Atom a --> Atom b)` `Atom a --> Atom b`;;
-check_conv TRANSL_CONV `TRANSL (p --> q)` `TRANSL p --> TRANSL q`;;
-check_conv TRANSL_CONV `TRANSL (Box (Atom a))` `Dotbox Atom a`;;
-check_conv TRANSL_CONV `TRANSL (Box (p --> Box q))`
-                       `Dotbox (TRANSL p --> Dotbox TRANSL q)`;;
+check_conv_eq TRANSL_CONV `TRANSL (Atom a)` `Atom a`;;
+check_conv_eq TRANSL_CONV `TRANSL True` `True`;;
+check_conv_eq TRANSL_CONV `TRANSL False` `False`;;
+check_conv_eq TRANSL_CONV `TRANSL (Not True)` `Not True`;;
+check_conv_eq TRANSL_CONV `TRANSL (Atom a --> Atom b)` `Atom a --> Atom b`;;
+check_conv_eq TRANSL_CONV `TRANSL (p --> q)` `TRANSL p --> TRANSL q`;;
+check_conv_eq TRANSL_CONV `TRANSL (Box (Atom a))` `Dotbox Atom a`;;
+check_conv_eq TRANSL_CONV `TRANSL (Box (p --> Box q))`
+                          `Dotbox (TRANSL p --> Dotbox TRANSL q)`;;
 
 (* ------------------------------------------------------------------------- *)
 (* Examples: Prove a formula of S4 via its tranlation in K4.                 *)
@@ -85,41 +65,6 @@ time HOLMS_RULE tm';; (* CPU time (user): 0.002222 *)
 
 g `!p. [S4_AX . {} |~ p] ==> [K4_AX . {} |~ TRANSL p]`;;
 (* TODO *)
-
-(* ------------------------------------------------------------------------- *)
-(* "God" translation: GOD (p --> q)  ~~>  Box (GOD p --> GOD q).             *)
-(* ------------------------------------------------------------------------- *)
-
-let GOD = define
-  `(!s. GOD (Atom s) = Box Atom s) /\
-   GOD True = Box True /\
-   GOD False = False /\
-   (!p. GOD (Not p) = Box Not (GOD p)) /\
-   (!p q. GOD (p && q) = GOD p && GOD q) /\
-   (!p q. GOD (p || q) = GOD p || GOD q) /\
-   (!p q. GOD (p --> q) = Box (GOD p --> GOD q)) /\
-   (!p q. GOD (p <-> q) = Box (GOD p --> GOD q) && Box (GOD q --> GOD p))`;;
-
-let GOD_CONV:conv = REWRITE_CONV[TRANSL; GOD];;
-
-(* ------------------------------------------------------------------------- *)
-(* Examples: Prove a formula of intuitionistic propositional logic           *)
-(* via its tranlation in GL.                                                 *)
-(* ------------------------------------------------------------------------- *)
-
-(* Example: Prove formula (p --> p). *)
-let tm = `[GL_AX . {} |~ TRANSL (GOD (Atom "p" --> Atom "p"))]`;;
-let tm' = run_conv GOD_CONV tm;;
-HOLMS_RULE tm';;
-
-(* Example: Excluded Middle (p || Not p) is not provable. *)
-let tm = `[GL_AX . {} |~ TRANSL (GOD (Atom "p" || Not Atom "p"))]`;;
-let tm' = run_conv GOD_CONV tm;;
-let tm' = subst [`p:form`,`Atom "p"`] tm';;
-let tm' = run_conv (REWRITE_CONV[dotbox_DEF]) tm';;
-HOLMS_RULE tm';;
-let ctm = HOLMS_BUILD_COUNTERMODEL tm';;
-GL_HOLMS_CERTIFY_COUNTERMODEL ctm tm';;
 
 (* ------------------------------------------------------------------------- *)
 (* ML function for modal formula translations (Box  ~~>  Dotbox).            *)
