ad_hoc_correspondence.ml
@@ -7,6 +7,8 @@
 (*                Cosimo Perini Brogi 2025.                                  *)
 (* ========================================================================= *)
 
+needs "HOLMS/calculus.ml";;
+
 (* ------------------------------------------------------------------------- *)
 (* Axiom Schemata.                                                           *)
 (* ------------------------------------------------------------------------- *)
@@ -18,32 +20,29 @@ let T_SCHEMA_DEF = new_definition
   `T_SCHEMA p = (Box p --> p)`;;
 
 let FOUR_SCHEMA_DEF = new_definition
-  `4_SCHEMA p = (Box p --> Box Box p)`;;
+  `FOUR_SCHEMA p = (Box p --> Box Box p)`;;
 
 let B_SCHEMA_DEF = new_definition
   `B_SCHEMA p = (p --> Box (Diam p))`;;
 
 let FIVE_SCHEMA_DEF = new_definition
-  `5_SCHEMA p = (Diam p --> Box Diam p)`;;
+   `FIVE_SCHEMA p = (Diam p --> Box Diam p)`;;
 
 let LOB_SCHEMA_DEF = new_definition
-  `LOB_SCHEMA p = (Box (Box p --> p) --> Box p)`;;
+  `LOB_SCHEMA p = Box (Box p --> p) --> Box p`;;
 
 (* ------------------------------------------------------------------------- *)
 (* Properties of Binary Relationship.                                        *)
 (* ------------------------------------------------------------------------- *)
 
 let SERIAL = new_definition
-  `SERIAL W R <=>
-   (!w:W. w IN W ==> ?y:W. y IN W /\ (R w y))`;;
+  `SERIAL W R <=> (!w:W. w IN W ==> ?y:W. y IN W /\ (R w y))`;;
 
 let REFLEXIVE = new_definition
-  `REFLEXIVE W R <=>
-   (!w:W. w IN W ==> R w w)`;;
+  `REFLEXIVE W R <=> (!w:W. w IN W ==> R w w)`;;
 
 let IRREFLEXIVE = new_definition
-  `IRREFLEXIVE W R <=>
-   (!x:W. x IN W ==> ~R x x)`;;
+  `IRREFLEXIVE W R <=> (!x:W. x IN W ==> ~R x x)`;;
 
 let TRANSITIVE = new_definition
   `TRANSITIVE W R <=>
@@ -51,11 +50,13 @@ let TRANSITIVE = new_definition
                  R w w' /\ R w' w''
                  ==> R w w'')`;;
 
-let SYMETRIC = new_definition
-  `SYMETRIC W R <=>
-   (!w w':W. w IN W /\ w' IN W /\
-             R w w'
-             ==> R w' w)`;;
+let SYMMETRIC = new_definition
+  `SYMMETRIC W R <=>
+   (!w w':W. w IN W /\ w' IN W /\ R w w' ==> R w' w)`;;
+
+let ANTISYMMETRIC = new_definition
+  `ANTISYMMETRIC W R <=>
+   (!w w':W. w IN W /\ w' IN W /\ R w w' /\ R w' w ==> w = w')`;;
 
 let EUCLIDEAN = new_definition
   `EUCLIDEAN W R <=>
@@ -68,52 +69,46 @@ let EUCLIDEAN = new_definition
 (* ------------------------------------------------------------------------- *)
 
 let MODAL_SER = prove
- (`!W:W->bool R.
-     SERIAL W R <=>
-     (!p. holds_in (W,R) (D_SCHEMA p))`,
-  REWRITE_TAC[diam_DEF; D_SCHEMA_DEF] THEN
-  MODAL_SCHEMA_TAC THEN MESON_TAC[SERIAL]);;
+ (`!W:W->bool R. SERIAL W R <=>
+                 (!p. holds_in (W,R) (D_SCHEMA p))`,
+  REWRITE_TAC[diam_DEF; D_SCHEMA_DEF] THEN MODAL_SCHEMA_TAC THEN
+  MESON_TAC[SERIAL]);;
 
 let MODAL_REFL = prove
- (`!W:W->bool R.
-     REFLEXIVE W R <=>
-     (!p. holds_in (W,R) (T_SCHEMA p))`,
-  REWRITE_TAC[REFLEXIVE; T_SCHEMA_DEF] THEN
-  MODAL_SCHEMA_TAC THEN MESON_TAC[]);;
+ (`!W:W->bool R. REFLEXIVE W R <=> (!p. holds_in (W,R) (T_SCHEMA p))`,
+  REWRITE_TAC[REFLEXIVE; T_SCHEMA_DEF] THEN MODAL_SCHEMA_TAC THEN
+  MESON_TAC[]);;
 
 let MODAL_TRANS = prove
- (`!W:W->bool R.
-     TRANSITIVE W R <=>
-     (!p. holds_in (W,R) (4_SCHEMA p))`,
+ (`!W:W->bool R. TRANSITIVE W R <=> (!p. holds_in (W,R) (FOUR_SCHEMA p))`,
   REWRITE_TAC[TRANSITIVE; FOUR_SCHEMA_DEF] THEN
   MODAL_SCHEMA_TAC THEN MESON_TAC[]);;
 
 let MODAL_SYM = prove
- (`!W:W->bool R.
-     SYMETRIC W R <=>
-     (!p. holds_in (W,R) (B_SCHEMA p))`,
-  ASM_REWRITE_TAC[diam_DEF; SYMETRIC; B_SCHEMA_DEF] THEN MODAL_SCHEMA_TAC THEN
+ (`!W:W->bool R. SYMMETRIC W R <=>
+                 (!p. holds_in (W,R) (B_SCHEMA p))`,
+  ASM_REWRITE_TAC[diam_DEF; SYMMETRIC; B_SCHEMA_DEF] THEN MODAL_SCHEMA_TAC THEN
   EQ_TAC THENL [ASM_MESON_TAC[]; REPEAT STRIP_TAC] THEN
   FIRST_X_ASSUM (MP_TAC o SPECL [`\v:W. v = w`; `w:W`]) THEN ASM_MESON_TAC[]);;
 
 let MODAL_EUCL = prove
- (`!W:W->bool R.
-      EUCLIDEAN W R <=>
-     (!p. holds_in (W,R) (5_SCHEMA p))`,
+ (`!W:W->bool R. EUCLIDEAN W R <=>
+                 (!p. holds_in (W,R) (FIVE_SCHEMA p))`,
   REWRITE_TAC[diam_DEF; EUCLIDEAN; FIVE_SCHEMA_DEF] THEN MODAL_SCHEMA_TAC THEN
   EQ_TAC THENL [ASM_MESON_TAC[]; REPEAT STRIP_TAC] THEN
   FIRST_X_ASSUM (MP_TAC o SPECL [`\v:W. v = w'`; `w:W`]) THEN
   ASM_MESON_TAC[]);;
 
 let MODAL_TRANSNT = prove
- (`!W:W->bool R. ((!x y. R x y ==> x IN W /\ y IN W) ==>
-      (TRANSITIVE W R /\ WF(\x y. R y x)  <=>
-      (!p. holds_in (W,R) (LOB_SCHEMA p))))`,
+ (`!W:W->bool R. (!x y. R x y ==> x IN W /\ y IN W)
+                 ==> (TRANSITIVE W R /\ WF(\x y. R y x) <=>
+                      !p. holds_in (W,R) (LOB_SCHEMA p))`,
   REWRITE_TAC[TRANSITIVE; LOB_SCHEMA_DEF] THEN MODAL_SCHEMA_TAC THEN
   DISCH_TAC THEN EQ_TAC THENL
   [INTRO_TAC "TRANS WF" THEN HYP_TAC "WF" (REWRITE_RULE[WF_IND]) THEN
    REPEAT GEN_TAC THEN REPEAT DISCH_TAC THEN FIRST_X_ASSUM MATCH_MP_TAC THEN
-   ASM_MESON_TAC[]; ALL_TAC] THEN
+   ASM_MESON_TAC[];
+   ALL_TAC] THEN
   INTRO_TAC "U" THEN CONJ_TAC THENL
   [X_GEN_TAC `w:W` THEN FIRST_X_ASSUM(MP_TAC o SPECL
    [`\v:W. v IN W /\ R w v /\ !w''. w'' IN W /\ R v w'' ==> R w w''`;
