god_transl.ml
@@ -1,0 +1,157 @@
+(* ========================================================================= *)
+(* Experiments with the "GOD" translation.                                   *)
+(*                                                                           *)
+(* (c) Copyright, Antonella Bilotta, Marco Maggesi,                          *)
+(*                Cosimo Perini Brogi 2026.                                  *)
+(* ========================================================================= *)
+
+needs "HOLMS/grz_tests.ml";;
+
+(* ------------------------------------------------------------------------- *)
+(* "God" translation: GOD (p --> q)  ~~>  Box (GOD p --> GOD q).             *)
+(* ------------------------------------------------------------------------- *)
+
+let GOD = define
+  `(!s. GOD (Atom s) = Box Atom s) /\
+   GOD True = Box True /\
+   GOD False = False /\
+   (!p. GOD (Not p) = Box Not (GOD p)) /\
+   (!p q. GOD (p && q) = GOD p && GOD q) /\
+   (!p q. GOD (p || q) = GOD p || GOD q) /\
+   (!p q. GOD (p --> q) = Box (GOD p --> GOD q)) /\
+   (!p q. GOD (p <-> q) = Box (GOD p --> GOD q) && Box (GOD q --> GOD p))`;;
+
+let GOD_TRANSL_CONV : conv = REWRITE_CONV[TRANSL; GOD];;
+
+(* ------------------------------------------------------------------------- *)
+(* Examples: Prove a formula of intuitionistic propositional logic           *)
+(* via its tranlation in GL.                                                 *)
+(* ------------------------------------------------------------------------- *)
+
+(* Example: Prove formula (p --> p). *)
+`[GRZ_AX . {} |~ GOD (Atom "p" --> Atom "p")]`
+|> run_conv GOD_TRANSL_CONV
+|> run_conv GRZ_CONV;;
+
+(* Example: Excluded Middle: (p || Not p) is not provable "in GOD". *)
+let tm = `[GL_AX . {} |~ TRANSL (GOD (Atom "p" || Not Atom "p"))]`;;
+let tm' = tm
+          |> run_conv GOD_TRANSL_CONV
+          |> run_conv (REWRITE_CONV[dotbox_DEF]);;
+check_conv_false GL_CONV tm';;
+(* Countermodel *)
+let ctm = !the_HOLMS_countermodel
+          |> vsubst[`R_PLUS (W:num->bool) R`,`R:num->num->bool`];;
+
+(* ------------------------------------------------------------------------- *)
+(* GOD tests.                                                                *)
+(* ------------------------------------------------------------------------- *)
+
+let mk_god_proves =
+  let grzv_tm = `[GRZ_AX . {} |~ GOD p]` in
+  fun tm -> let tm' = vsubst ipatoms tm in
+            vsubst [tm',ptm] grzv_tm;;
+
+let GOD_CONV = PURE_REWRITE_CONV[GOD] THENC GRZ_CONV;;
+let test_god_proves = check_conv_true GOD_CONV o mk_god_proves;;
+let test_god_disproves = check_conv_false GOD_CONV o mk_god_proves;;
+
+(* Proves. *)
+test_god_proves `p --> q || q --> p`;;
+test_god_disproves `q || (q --> (p || Not q))`;;
+(* Questi sotto non terminano (provati per circa 30min)! *)
+(* test_god_proves `(q --> p) --> (Not p --> Not q)`;; *)
+(* test_god_proves `(Not p --> q || r) --> (Not p --> q) || (Not p --> r)`;; *)
+
+(* Disproves. *)
+test_god_disproves `p || Not p`;;
+test_god_disproves `Not Not p --> p`;;
+(* Questi sotto non terminano (provati per circa 30min)! *)
+(* test_god_disproves `(Not p --> Not q) --> (q --> p)`;; *)
+
+(* ************************************************************************* *)
+(* ************************************************************************* *)
+(*                                                                           *)
+(*                     Size of the unctractable terms                        *)
+(*                                                                           *)
+(* ************************************************************************* *)
+(* ************************************************************************* *)
+
+let swap (x,y) = (y,x);;
+
+(* ------------------------------------------------------------------------- *)
+(* First example (reversed contrapositive):                                  *)
+(* (Not p --> Not q) --> (q --> p)                                           *)
+(* ------------------------------------------------------------------------- *)
+
+g `[GRZ_AX . {} |~ GOD ((Not Atom "p" --> Not Atom "q")
+                        --> (Atom "q" --> Atom "p"))]`;;
+e (REWRITE_TAC[GOD]);;
+(* e (CONV_TAC GRZ_CONV);; *)
+e (CONV_TAC (GEN_REWRITE_CONV I [GRZ_TRANSL]));;
+e (CONV_TAC (GEN_REWRITE_CONV (RAND_CONV o TOP_DEPTH_CONV)
+                              [TRANSL; diam_DEF; dotbox_DEF]));;
+(* e GL_TAC;; *)
+
+`(Not p --> Not q) --> (q --> p)`
+|> mk_god_proves
+|> run_conv (REWRITE_CONV[GOD; GRZ_TRANSL; TRANSL; diam_DEF; dotbox_DEF])
+|> rand
+|> subst (map swap ipatoms)
+;;
+
+(*
+val tm : term =
+  `Box (Box (Box Not (Box p && p) && Not (Box p && p) -->
+             Box Not (Box q && q) && Not (Box q && q)) &&
+        (Box Not (Box p && p) && Not (Box p && p) -->
+         Box Not (Box q && q) && Not (Box q && q)) -->
+        Box (Box q && q --> Box p && p) && (Box q && q --> Box p && p)) &&
+   (Box (Box Not (Box p && p) && Not (Box p && p) -->
+         Box Not (Box q && q) && Not (Box q && q)) &&
+    (Box Not (Box p && p) && Not (Box p && p) -->
+     Box Not (Box q && q) && Not (Box q && q)) -->
+    Box (Box q && q --> Box p && p) && (Box q && q --> Box p && p))`
+*)
+
+(* ------------------------------------------------------------------------- *)
+(* Second example:                                                           *)
+(* (Not p --> q || r) --> (Not p --> q) || (Not p --> r)                     *)
+(* ------------------------------------------------------------------------- *)
+
+g `[GRZ_AX . {} |~
+    GOD ((Not Atom "p" --> Atom "q" || Atom"r")
+         --> (Not Atom "p" --> Atom "q") ||
+             (Not Atom "p" --> Atom"r"))]`;;
+e (REWRITE_TAC[GOD]);;
+(* e (CONV_TAC GRZ_CONV);; *)
+e (CONV_TAC (GEN_REWRITE_CONV I [GRZ_TRANSL]));;
+e (CONV_TAC (GEN_REWRITE_CONV (RAND_CONV o TOP_DEPTH_CONV)
+                              [TRANSL; diam_DEF; dotbox_DEF]));;
+(* e GL_TAC;; *)
+
+`(Not p --> q || r) --> (Not p --> q) || (Not p --> r)`
+|> mk_god_proves
+|> run_conv (REWRITE_CONV[GOD; GRZ_TRANSL; TRANSL; diam_DEF; dotbox_DEF])
+|> rand
+|> subst (map swap ipatoms)
+;;
+
+(*
+val it : term =
+  `Box (Box (Box Not (Box p && p) && Not (Box p && p) -->
+             Box q && q || Box r && r) &&
+        (Box Not (Box p && p) && Not (Box p && p) -->
+         Box q && q || Box r && r) -->
+        Box (Box Not (Box p && p) && Not (Box p && p) --> Box q && q) &&
+        (Box Not (Box p && p) && Not (Box p && p) --> Box q && q) ||
+        Box (Box Not (Box p && p) && Not (Box p && p) --> Box r && r) &&
+        (Box Not (Box p && p) && Not (Box p && p) --> Box r && r)) &&
+   (Box (Box Not (Box p && p) && Not (Box p && p) -->
+         Box q && q || Box r && r) &&
+    (Box Not (Box p && p) && Not (Box p && p) --> Box q && q || Box r && r) -->
+    Box (Box Not (Box p && p) && Not (Box p && p) --> Box q && q) &&
+    (Box Not (Box p && p) && Not (Box p && p) --> Box q && q) ||
+    Box (Box Not (Box p && p) && Not (Box p && p) --> Box r && r) &&
+    (Box Not (Box p && p) && Not (Box p && p) --> Box r && r))`
+*)
