grz.ml
@@ -1,0 +1,1374 @@
+(* ========================================================================= *)
+(* Grzegorczyk Logic (Grz).                                                  *)
+(*                                                                           *)
+(* Meta-theory (soundness and completeness).                                 *)
+(* Translation to GL Logic.                                                  *)
+(* Decision procedure via the translation.                                   *)
+(*                                                                           *)
+(* (c) Copyright, Antonella Bilotta, Marco Maggesi,                          *)
+(*                Cosimo Perini Brogi 2025-26.                               *)
+(* ========================================================================= *)
+
+needs "HOLMS/k_decid.ml";;       (* Used in GRZ_EQ_S4GRZ and its lemmas     *)
+needs "HOLMS/s4_decid.ml";;      (* Used in S4GRZ_TRUTH_LEMMA               *)
+needs "HOLMS/gl_decid.ml";;      (* Used in GRZ_TAC                         *)
+needs "HOLMS/translations.ml";;
+
+(* ------------------------------------------------------------------------- *)
+(* 1. Axiomatic presentations of Grzegorczyk.                                *)
+(* ------------------------------------------------------------------------- *)
+
+(* ------------------------------------------------------------------------- *)
+(* Definition of the axiomatic calculus Grz.                                 *)
+(* ------------------------------------------------------------------------- *)
+
+let GRZ_SCHEMA_DEF = new_definition
+  `GRZ_SCHEMA p = (Box (Box (p --> Box p) --> p) --> p)`;;
+
+let GRZ_AX = new_definition
+  `GRZ_AX = {GRZ_SCHEMA p| p IN (:form)}`;;
+
+let GRZ_IN_GRZ_AX = prove
+ (`!p. Box (Box (p --> Box p) --> p) --> p IN GRZ_AX`,
+  REWRITE_TAC[GRZ_AX; GRZ_SCHEMA_DEF; IN_ELIM_THM; IN_UNIV] THEN MESON_TAC[]);;
+
+let GRZ_AX_GRZ = prove
+ (`!p. [GRZ_AX. {} |~ Box (Box (p --> Box p) --> p) --> p]`,
+  MESON_TAC[MODPROVES_RULES; GRZ_IN_GRZ_AX]);;
+
+(* ------------------------------------------------------------------------- *)
+(* Definition of the axiomatic calculus S4GRZ.                               *)
+(* ------------------------------------------------------------------------- *)
+
+let S4GRZ_AX = new_definition
+  `S4GRZ_AX = {FOUR_SCHEMA p| p IN (:form)} UNION
+              {T_SCHEMA p |p IN (:form)} UNION
+              {GRZ_SCHEMA p| p IN (:form)}`;;
+
+let GRZ_IN_S4GRZ_AX = prove
+ (`!p. Box (Box (p --> Box p) --> p) --> p IN S4GRZ_AX`,
+  REWRITE_TAC[S4GRZ_AX; GRZ_SCHEMA_DEF; IN_ELIM_THM; IN_UNIV; UNION] THEN
+  MESON_TAC[]);;
+
+let S4GRZ_AX_GRZ = prove
+ (`!p. [S4GRZ_AX. {} |~ Box (Box (p --> Box p) --> p) --> p]`,
+  MESON_TAC[MODPROVES_RULES; GRZ_IN_S4GRZ_AX]);;
+
+(* ------------------------------------------------------------------------- *)
+(* Proof of the equivalence between Grz and S4GRZ.                           *)
+(* See Boolos §12 p.157-158.                                                 *)
+(* ------------------------------------------------------------------------- *)
+
+let GRZ_PROVES_T = prove
+ (`!H p. [GRZ_AX . H |~ T_SCHEMA p]`,
+  REPEAT GEN_TAC THEN MATCH_MP_TAC MODPROVES_MONO2 THEN
+  EXISTS_TAC `{}:form->bool` THEN
+  REWRITE_TAC[EMPTY_SUBSET; T_SCHEMA_DEF] THEN
+  MATCH_MP_TAC MLK_imp_trans THEN
+  EXISTS_TAC `Box (Box (p --> Box p) --> p)` THEN
+  CONJ_TAC THENL
+  [MATCH_MP_TAC MODPROVES_MONO1 THEN
+   EXISTS_TAC `{}:form->bool` THEN
+   CONJ_TAC THENL [ASM_MESON_TAC[EMPTY_SUBSET]; HOLMS_TAC];
+   ASM_MESON_TAC[MODPROVES_RULES; GRZ_IN_GRZ_AX]]);;
+
+let GRZ_PROVES_4 = prove
+ (`!H p.[GRZ_AX . H |~ FOUR_SCHEMA p]`,
+  REPEAT GEN_TAC THEN MATCH_MP_TAC MODPROVES_MONO2 THEN
+  EXISTS_TAC `{}:form->bool` THEN
+  REWRITE_TAC[EMPTY_SUBSET; FOUR_SCHEMA_DEF] THEN
+  ABBREV_TAC `C = (FOUR_SCHEMA p) && p` THEN MATCH_MP_TAC MLK_frege THEN
+  EXISTS_TAC `Box p` THEN CONJ_TAC THENL
+  [MATCH_MP_TAC MLK_imp_trans THEN EXISTS_TAC `C:form` THEN CONJ_TAC THENL
+   [MATCH_MP_TAC MLK_imp_trans THEN
+    EXISTS_TAC `Box (Box (C --> Box C) --> C)` THEN CONJ_TAC THENL
+    [MATCH_MP_TAC MODPROVES_MONO1 THEN EXISTS_TAC `{}:form->bool` THEN
+     CONJ_TAC THENL
+      [MESON_TAC[EMPTY_SUBSET];
+       EXPAND_TAC "C" THEN RULE_ASSUM_TAC SYM THEN
+       ASM_REWRITE_TAC[FOUR_SCHEMA_DEF] THEN HOLMS_TAC];
+     ASM_MESON_TAC[MODPROVES_RULES; GRZ_IN_GRZ_AX; FOUR_SCHEMA_DEF]];
+    ASM_MESON_TAC[MLK_and_left_th; FOUR_SCHEMA_DEF]];
+   ASM_MESON_TAC[MODPROVES_RULES; KAXIOM_RULES; FOUR_SCHEMA_DEF]]);;
+
+let S4GRZ_prove_S4 = prove
+ (`!H p. [S4_AX . H |~ p] ==> [S4GRZ_AX . H |~ p]`,
+  REPEAT GEN_TAC THEN DISCH_TAC THEN MATCH_MP_TAC MODPROVES_MONO1 THEN
+  EXISTS_TAC `S4_AX` THEN ASM_REWRITE_TAC[S4GRZ_AX; S4_AX] THEN SET_TAC[]);;
+
+let GRZ_EQ_S4GRZ = prove
+ (`!H p. [GRZ_AX . H |~ p] <=> [S4GRZ_AX . H |~ p]`,
+  REPEAT GEN_TAC THEN EQ_TAC THENL
+  [DISCH_TAC THEN MATCH_MP_TAC MODPROVES_MONO1 THEN EXISTS_TAC `GRZ_AX` THEN
+   CONJ_TAC THENL [SET_TAC[GRZ_AX; S4GRZ_AX]; ASM_REWRITE_TAC[]];
+   SUBGOAL_THEN `!H p. [S4GRZ_AX . H |~ p] ==> [GRZ_AX . H |~ p]` MP_TAC THENL
+   [MATCH_MP_TAC MODPROVES_INDUCT THEN REPEAT CONJ_TAC THENL
+    [MESON_TAC[MODPROVES_RULES];
+     REWRITE_TAC[IN_ELIM_THM; S4GRZ_AX; IN_UNION] THEN REPEAT STRIP_TAC THENL
+     [ASM_MESON_TAC[GRZ_PROVES_4];
+      ASM_MESON_TAC[GRZ_PROVES_T];
+      ASM_MESON_TAC[EMPTY_SUBSET; MODPROVES_RULES;
+                    GRZ_IN_GRZ_AX; GRZ_SCHEMA_DEF]];
+     MESON_TAC[MODPROVES_RULES];
+     MESON_TAC[MODPROVES_RULES];
+     MESON_TAC[MODPROVES_RULES]];
+    MESON_TAC[]]]);;
+
+(* ------------------------------------------------------------------------- *)
+(* 2. Semantic presentations of Grzegorczyk.                                 *)
+(* ------------------------------------------------------------------------- *)
+
+(* ------------------------------------------------------------------------- *)
+(* Alternative characterization for posets.                                  *)
+(* ------------------------------------------------------------------------- *)
+
+let POSET_EQ = prove
+ (`!(<<) W.
+     poset (<<) /\ fld (<<) = W <=>
+     (!x y:W. x << y ==> x IN W /\ y IN W) /\
+     REFLEXIVE W (<<) /\
+     TRANSITIVE W (<<) /\
+     ANTISYMMETRIC W (<<)`,
+  REWRITE_TAC[poset; REFLEXIVE; TRANSITIVE; ANTISYMMETRIC;
+              EXTENSION; SUBSET] THEN
+  MESON_TAC[IN_FLD]);;
+
+(* ------------------------------------------------------------------------- *)
+(* Definition of weakly wellfoundedness for arbitrary (infix) relation <<    *)
+(* ------------------------------------------------------------------------- *)
+(* ------------------------------------------------------------------------- *)
+(* Modified WWF: restricts quantification on `P SUBSET fld`.                 *)
+(* ------------------------------------------------------------------------- *)
+
+let WWF = new_definition
+  `WWF (<<) <=>
+   (!P. (?x:W. P x) /\ (!x. P x ==> x IN fld (<<))
+        ==> (?x. P x /\ (!y. ~(x = y) /\ y << x ==> ~P y)))`;;
+
+let WWF_EQ = prove
+ (`!(<<). WWF (<<) <=>
+          !P. (!x. P x ==> x IN fld (<<))
+              ==> ((?x:A. P(x)) <=>
+                   (?x. P(x) /\ (!y. ~(x = y) /\ y << x ==> ~P(y))))`,
+  GEN_TAC THEN REWRITE_TAC[WWF] THEN EQ_TAC THENL
+  [MESON_TAC[];
+   INTRO_TAC "hp; !P; ne sub" THEN
+   HYP_TAC "hp: +" (SPEC `P:A->bool`) THEN
+   ASM_MESON_TAC[]]);;
+
+let WWF_IND = prove
+ (`!(<<). WWF(<<) <=>
+          !P. (!x:A. ~P x ==> x IN fld (<<))
+              ==> (!x. (!y. y << x /\ ~(x = y) ==> P y) ==> P x) ==> !x. P x`,
+  GEN_TAC THEN REWRITE_TAC[WWF] THEN EQ_TAC THEN REPEAT STRIP_TAC THEN
+  FIRST_X_ASSUM(MP_TAC o SPEC `\x:A. ~P(x)`) THEN BETA_TAC THEN
+  ASM_MESON_TAC[]);;
+
+(* ------------------------------------------------------------------------- *)
+(* Equivalent formualtion.                                                   *)
+(* ------------------------------------------------------------------------- *)
+
+let WWF_ALT = prove
+ (`!l. WWF l <=>
+       (!s. ~(s = {}) /\ s SUBSET fld l
+            ==> (?a:W. a IN s /\ (!x. x IN s ==> ~properly l x a)))`,
+  REWRITE_TAC[WWF; properly; SUBSET; IN; GSYM MEMBER_NOT_EMPTY] THEN
+  MESON_TAC[]);;
+
+(* ------------------------------------------------------------------------- *)
+(* Finite non-empty posets are WWF (specialization of POSET_MAX).            *)
+(* ------------------------------------------------------------------------- *)
+
+let POSET_WWF = prove
+ (`!l:A->A->bool. poset l /\ ~(fld l = {}) /\ FINITE (fld l) ==> WWF l`,
+  INTRO_TAC "!l; l ne fin" THEN REWRITE_TAC[WWF_ALT] THEN
+  MP_TAC (ISPECL [`l:A->A->bool`] POSET_MIN) THEN
+  INTRO_TAC "max; !s; ne sub" THEN
+  HYP_TAC "max: +" (SPEC `s:A->bool`) THEN ANTS_TAC THENL
+  [ASM_REWRITE_TAC[] THEN
+   ASM_MESON_TAC[FINITE_SUBSET];
+   ASM_MESON_TAC[]]);;
+
+let POSET_WWF_ALT = prove
+ (`!(<<) W. (!x y:W. x << y ==> x IN W /\ y IN W) /\
+            REFLEXIVE W (<<) /\
+            TRANSITIVE W (<<) /\
+            ANTISYMMETRIC W (<<) /\
+            FINITE W /\
+            ~(W = {})
+            ==> WWF (<<)`,
+  REPEAT STRIP_TAC THEN MATCH_MP_TAC POSET_WWF THEN ASM_MESON_TAC[POSET_EQ]);;
+
+(* ------------------------------------------------------------------------- *)
+(* Reflexive, Transitive and Weakly Noetherian Frames.                       *)
+(* ------------------------------------------------------------------------- *)
+
+let RTWN_DEF = new_definition
+  `RTWN =
+   {(W:W->bool,R:W->W->bool) |
+    (W,R) IN FRAME /\
+    REFLEXIVE W R /\
+    TRANSITIVE W R /\
+    WWF (\x y. R y x)}`;;
+
+let IN_RTWN = prove
+ (`(W:W->bool,R:W->W->bool) IN RTWN <=>
+   (W,R) IN FRAME /\
+   REFLEXIVE W R /\
+   TRANSITIVE W R /\
+   WWF (\x y. R y x)`,
+  REWRITE_TAC[RTWN_DEF; IN_ELIM_PAIR_THM]);;
+
+(* ------------------------------------------------------------------------- *)
+(* Reflexive, Antisymmetric, Transitive Finite Frames.                       *)
+(* ------------------------------------------------------------------------- *)
+
+let RATF_DEF = new_definition
+ `RATF =
+  {(W:W->bool,R:W->W->bool) |
+   FINITE_FRAME (W,R) /\
+   REFLEXIVE W R /\
+   TRANSITIVE W R /\
+   ANTISYMMETRIC W R}`;;
+
+let IN_RATF = prove
+ (`(W:W->bool,R:W->W->bool) IN RATF <=>
+   (W,R) IN FINITE_FRAME /\
+   REFLEXIVE W R /\
+   TRANSITIVE W R /\
+   ANTISYMMETRIC W R`,
+  MESON_TAC[RATF_DEF; IN_ELIM_PAIR_THM; IN]);;
+
+(* ------------------------------------------------------------------------- *)
+(* RATFs Frames are RTWN Frames.                                             *)
+(* ------------------------------------------------------------------------- *)
+
+let RATF_SUBSET_RTWN = prove
+ (`(RATF:(W->bool)#(W->W->bool)->bool ) SUBSET RTWN`,
+  REWRITE_TAC[SUBSET; IN_RATF; IN_RTWN; FORALL_PAIR_THM;
+              IN_FRAME; IN_FINITE_FRAME] THEN
+  INTRO_TAC "![W] [R]; (non_empty (rel finite)) refl trans antisym" THEN
+  ASM_REWRITE_TAC[] THEN
+  MATCH_MP_TAC POSET_WWF_ALT THEN
+  EXISTS_TAC `W:W->bool` THEN ASM_REWRITE_TAC[] THEN
+  HYP (MP_TAC o end_itlist CONJ) "rel refl trans antisym" [] THEN
+  REWRITE_TAC[REFLEXIVE; TRANSITIVE; ANTISYMMETRIC] THEN
+  MESON_TAC[]);;
+
+(* ------------------------------------------------------------------------- *)
+(* 3. Soundness Lemmas.                                                      *)
+(* ------------------------------------------------------------------------- *)
+
+(* ------------------------------------------------------------------------- *)
+(* Correspondence Theory: RTWN Frames are characteristic for S4GRZ.          *)
+(* ------------------------------------------------------------------------- *)
+
+let MODAL_RTWN = prove
+ (`!W:W->bool R.
+     (!x y. R x y ==> x IN W /\ y IN W)
+     ==> REFLEXIVE W R /\ TRANSITIVE W R /\ WWF (\x y. R y x)
+     ==> !p. holds_in (W,R) (GRZ_SCHEMA p)`,
+  REWRITE_TAC[REFLEXIVE; TRANSITIVE; GRZ_SCHEMA_DEF] THEN
+  INTRO_TAC "!W R; wd" THEN
+  INTRO_TAC "REFL TRANS WWF" THEN
+  HYP_TAC "WWF" (REWRITE_RULE[WWF_IND]) THEN
+  GEN_TAC THEN
+  ASM_REWRITE_TAC[holds_in] THEN
+  REPEAT GEN_TAC THEN
+  ABBREV_TAC `X_0 = {w:W | w IN W /\
+                           holds (W,R) V (Box (Box (p --> Box p) --> p)) w /\
+                           ~(holds (W,R) V p w)}` THEN
+  ABBREV_TAC `X_1 = {w:W | w IN W /\
+                           holds (W,R) V (Box (Box (p --> Box p) --> p)) w /\
+                           ~(holds (W,R) V (Box p) w) /\
+                           holds (W,R) V p w}` THEN
+  CLAIM_TAC "EMPTY_IN" `(X_0 INTER X_1) = {}:W->bool` THENL
+  [REFUTE_THEN MP_TAC THEN DISCH_TAC THEN
+   SUBGOAL_THEN `?x. x:W IN X_0 INTER X_1` MP_TAC THENL
+   [ASM_REWRITE_TAC[MEMBER_NOT_EMPTY]; ALL_TAC] THEN
+   INTRO_TAC "@x. NON_EMPTY" THEN
+   HYP_TAC "NON_EMPTY" (REWRITE_RULE[IN_INTER]) THEN
+   SUBGOAL_THEN `~(holds (W,R) V p (x:W)) /\ (holds (W,R) V p (x:W))`
+     MP_TAC THENL
+   [SUBGOAL_THEN `(x:W) IN
+                    {w:W | w IN W /\
+                           holds (W,R) V (Box (Box (p --> Box p) --> p)) w /\
+                           ~(holds (W,R) V p w)} /\
+                    x IN
+                     {w:W | w IN W /\
+                            holds (W,R) V (Box (Box (p --> Box p) --> p)) w /\
+                            ~(holds (W,R) V (Box p) w) /\ holds (W,R) V p w}`
+                  MP_TAC THENL
+     [ASM_MESON_TAC[]; ASM_REWRITE_TAC[IN_ELIM_THM] THEN ASM_MESON_TAC[]];
+    ASM_MESON_TAC[]];
+   DISCH_TAC] THEN
+  CLAIM_TAC "EMPTY_X0" `(X_0:W->bool) = {}` THENL
+  [CLAIM_TAC "w'_IN_X0_THEN_x_IN_X1"
+    `!w'. w' IN (X_0:W->bool) ==> ?x. ((R:W->W->bool) w' x /\ x IN X_1)` THENL
+   [REPEAT STRIP_TAC THEN
+    SUBGOAL_THEN `(w':W) IN
+                  {w | w IN W /\
+                       holds (W,R) V (Box (Box (p --> Box p) --> p)) w /\
+                       ~(holds (W,R) V p w)} ` MP_TAC THENL
+    [ASM_MESON_TAC[]; ALL_TAC] THEN
+    ASM_REWRITE_TAC[IN_ELIM_THM] THEN
+    INTRO_TAC "IN_X0_THEN_IN_W IN_X0_THEN_ForA IN_X0_THEN_NonForB" THEN
+    CLAIM_TAC "IN_X0_THEN_REFL" `((R:W->W->bool) w' w')` THENL
+    [ASM_MESON_TAC[]; ALL_TAC] THEN
+    CLAIM_TAC "For1" `holds (W,R) V (Box (p --> Box p) --> p) (w':W)` THENL
+    [SUBGOAL_THEN `holds (W,R) V (Box (Box (p --> Box p) --> p)) (w':W)`
+       MP_TAC THENL
+     [ASM_REWRITE_TAC[];
+      MODAL_SCHEMA_TAC THEN DISCH_TAC THEN FIRST_X_ASSUM MATCH_MP_TAC THEN
+      ASM_REWRITE_TAC[]];
+      ALL_TAC] THEN
+    CLAIM_TAC "Not_For2" `~ holds (W,R) V (Box (p --> Box p)) (w':W)` THENL
+    [SUBGOAL_THEN `~holds (W,R) V p (w':W) /\
+                    holds (W,R) V (Box (p --> Box p) --> p) (w':W)` MP_TAC THENL
+      [ASM_MESON_TAC[]; MODAL_SCHEMA_TAC THEN ASM_MESON_TAC[]];
+     ALL_TAC] THEN
+    SUBGOAL_THEN `?x. ((R:W->W->bool) w' x /\ holds (W,R) V (p) (x:W) /\
+                       ~holds (W,R) V (Box p) (x:W))` MP_TAC THENL
+    [SUBGOAL_THEN `~holds (W,R) V (Box (p --> Box p)) (w':W)` MP_TAC THENL
+     [ASM_MESON_TAC[];
+      MODAL_SCHEMA_TAC THEN ASM_REWRITE_TAC[NOT_FORALL_THM; NOT_IMP] THEN
+      INTRO_TAC "@z. a b @k. c" THEN EXISTS_TAC `z:W` THEN
+      REPEAT CONJ_TAC THEN ASM_MESON_TAC[]];
+     ALL_TAC] THEN
+    INTRO_TAC "@x. REL_x p Not_Box_p" THEN EXISTS_TAC `(x:W)` THEN
+    ASM_REWRITE_TAC[] THEN
+    SUBGOAL_THEN
+      `(x:W) IN {w | w IN W /\
+                     holds (W,R) V (Box (Box (p --> Box p) --> p)) w /\
+                     ~holds (W,R) V (Box p) w /\ holds (W,R) V p w}`
+      MP_TAC THENL
+    [ASM_REWRITE_TAC[IN_ELIM_THM] THEN CONJ_TAC THENL
+     [ASM_MESON_TAC[];
+      SUBGOAL_THEN `!z:W. R x z ==> holds (W,R) V (Box (p --> Box p) --> p) z`
+        MP_TAC THENL
+      [GEN_TAC THEN DISCH_TAC THEN CLAIM_TAC "REL_z" `(R:W->W->bool) w' z` THENL
+       [ASM_MESON_TAC[];
+        SUBGOAL_THEN `holds (W,R) V (Box (Box (p --> Box p) --> p)) (w':W)`
+          MP_TAC THENL
+        [ASM_REWRITE_TAC[];
+         MODAL_SCHEMA_TAC THEN DISCH_TAC THEN FIRST_X_ASSUM MATCH_MP_TAC THEN
+         ASM_MESON_TAC[]]];
+        MODAL_SCHEMA_TAC THEN ASM_MESON_TAC[]]];
+     ASM_MESON_TAC[]];
+    ALL_TAC] THEN
+   CLAIM_TAC "w'_IN_X1_THEN_x_IN_X0 "
+              `! w'. w' IN (X_1:W->bool) ==>
+                     ?x. ((R:W->W->bool) w' x /\ x IN X_0)` THENL
+    [REPEAT STRIP_TAC THEN
+     SUBGOAL_THEN `(w':W) IN
+                     {w | w IN W /\
+                          holds (W,R) V (Box (Box (p --> Box p) --> p)) w /\
+                          ~holds (W,R) V (Box p) w /\ holds (W,R) V p w} ` MP_TAC THENL
+      [ASM_MESON_TAC[]; ALL_TAC] THEN
+     ASM_REWRITE_TAC[IN_ELIM_THM] THEN
+     INTRO_TAC "IN_X1_THEN_IN_W IN_X1_THEN_ForA IN_X1_THEN_NonForB IN_X1_THEN_ForC" THEN
+     SUBGOAL_THEN `?x. (R:W->W->bool) w' x /\ ~holds (W,R) V p (x:W)` MP_TAC THENL
+      [SUBGOAL_THEN `~holds (W,R) V (Box p) (w':W)` MP_TAC THENL
+        [ASM_MESON_TAC[]; MODAL_SCHEMA_TAC THEN ASM_REWRITE_TAC[NOT_FORALL_THM; NOT_IMP] THEN
+         INTRO_TAC "@z. (a b) c" THEN EXISTS_TAC `z:W` THEN ASM_MESON_TAC[]];
+       ALL_TAC] THEN
+     INTRO_TAC "@x. REL_x Not_p" THEN EXISTS_TAC `(x:W)` THEN ASM_REWRITE_TAC[] THEN
+     SUBGOAL_THEN `(x:W) IN
+                   {w | w IN W /\
+                        holds (W,R) V (Box (Box (p --> Box p) --> p)) w /\
+                        ~(holds (W,R) V p w)}` MP_TAC THENL
+     [ASM_REWRITE_TAC[IN_ELIM_THM] THEN CONJ_TAC THENL
+      [ASM_MESON_TAC[];
+       SUBGOAL_THEN `!z. R x z ==> (holds (W,R) V (Box (p --> Box p) --> p) (z:W))` MP_TAC THENL
+       [GEN_TAC THEN DISCH_TAC THEN CLAIM_TAC "REL_z" `(R:W->W->bool) w' z` THENL
+        [ASM_MESON_TAC[];
+         SUBGOAL_THEN `holds (W,R) V (Box (Box (p --> Box p) --> p)) (w':W)` MP_TAC THENL
+         [ASM_REWRITE_TAC[]; MODAL_SCHEMA_TAC THEN DISCH_TAC THEN
+          FIRST_X_ASSUM MATCH_MP_TAC THEN ASM_MESON_TAC[]]];
+        MODAL_SCHEMA_TAC THEN ASM_MESON_TAC[]]];
+      ASM_MESON_TAC[]];
+     ALL_TAC] THEN
+   ABBREV_TAC `(X:W->bool) = X_0 UNION X_1` THEN
+   CLAIM_TAC "EMPTY_UN" `(X:W->bool) = {}` THENL
+    [SUBGOAL_THEN `WWF (\x y. (R:W->W->bool) y x)` MP_TAC THENL
+      [ASM_MESON_TAC[WWF_IND]; ALL_TAC] THEN
+     REWRITE_TAC[WWF_EQ] THEN DISCH_TAC THEN
+     FIRST_X_ASSUM (MP_TAC o SPEC `(\x:W. x IN X)`) THEN
+     REWRITE_TAC[IN_FLD] THEN ANTS_TAC THENL
+      [REWRITE_TAC[IN_FLD] THEN CLAIM_TAC "+" `X:W->bool SUBSET W` THENL
+        [MAP_EVERY EXPAND_TAC ["X"; "X_0"; "X_1"] THEN SET_TAC[]; HYP SET_TAC "REFL" []];
+       DISCH_TAC] THEN
+     SUBGOAL_THEN `~ ?x. x:W IN X` MP_TAC THENL
+      [ASM_REWRITE_TAC[] THEN
+       ASM_REWRITE_TAC[MEMBER_NOT_EMPTY;
+                       NOT_EXISTS_THM; DE_MORGAN_THM; NOT_FORALL_THM; NOT_IMP] THEN
+       REWRITE_TAC[TAUT `(~p \/ q) <=> (p ==> q)`] THEN GEN_TAC THEN DISCH_TAC THEN
+       SUBGOAL_THEN `(x:W IN X_0 \/ x IN X_1) /\ ~(x IN X_0 /\ x IN X_1)` MP_TAC THENL
+        [ASM_MESON_TAC[IN_UNION; DISJOINT; IN_DISJOINT]; ALL_TAC] THEN
+       STRIP_TAC THENL
+        [SUBGOAL_THEN `(?y. (R:W->W->bool) x y /\ y IN X_1)` MP_TAC THENL
+          [ASM_MESON_TAC[]; INTRO_TAC "@y. REL IN" THEN EXISTS_TAC `y:W` THEN
+           ASM_REWRITE_TAC[] THEN ASM_MESON_TAC[IN_UNION]];
+         SUBGOAL_THEN `(?y. (R:W->W->bool) x y /\ y IN X_0)` MP_TAC THENL
+          [ASM_MESON_TAC[]; INTRO_TAC "@y. REL IN" THEN EXISTS_TAC `y:W` THEN
+           ASM_REWRITE_TAC[] THEN ASM_MESON_TAC[IN_UNION]]];
+       ASM_MESON_TAC[MEMBER_NOT_EMPTY]];
+     ASM_MESON_TAC[EMPTY_UNION]];
+   ALL_TAC] THEN
+  SUBGOAL_THEN `~(?x. x IN {w | w IN (W:W->bool) /\
+                      holds (W,R) V (Box (Box (p --> Box p) --> p)) w /\
+                      ~holds (W,R) V p w})` MP_TAC THENL
+  [ASM_MESON_TAC[MEMBER_NOT_EMPTY]; ALL_TAC] THEN
+  REWRITE_TAC[IN_ELIM_THM] THEN DISCH_TAC THEN
+  REFUTE_THEN MP_TAC THEN DISCH_TAC THEN
+  SUBGOAL_THEN `?(x:W). (holds (W,R) V (Box (Box (p --> Box p) --> p)) x /\
+                         ~holds (W,R) V p x) /\
+                        x IN W` MP_TAC THENL
+  [UNDISCH_TAC `~holds (W,R) V (Box (Box (p --> Box p) --> p) --> p) (w:W)` THEN
+   MODAL_SCHEMA_TAC THEN ASM_REWRITE_TAC[NOT_FORALL_THM; NOT_IMP] THEN
+   DISCH_TAC THEN EXISTS_TAC `w:W` THEN
+   CONJ_TAC THENL [ASM_MESON_TAC[]; ALL_TAC] THEN
+   ASM_MESON_TAC[];
+   ASM_MESON_TAC[]]);;
+
+let RTWN_SUBSET_CHAR_S4GRZ = prove
+ (`RTWN:(W->bool)#(W->W->bool)->bool SUBSET CHAR S4GRZ_AX`,
+  REWRITE_TAC[SUBSET; FORALL_PAIR_THM; IN_CHAR; IN_RTWN] THEN
+  REWRITE_TAC[S4GRZ_AX; FORALL_IN_UNION; FORALL_IN_GSPEC; IN_UNIV] THEN
+  REPEAT STRIP_TAC THENL
+  [ASM_REWRITE_TAC[];
+   ASM_MESON_TAC[MODAL_TRANS];
+   ASM_MESON_TAC[MODAL_REFL];
+   ASM_MESON_TAC[MODAL_RTWN; IN_FRAME]]);;
+
+(* ------------------------------------------------------------------------- *)
+(* Soundness Lemma for S4GRZ.                                                *)
+(* ------------------------------------------------------------------------- *)
+
+let S4GRZ_RTWN_VALID = prove
+ (`!H p. [S4GRZ_AX . H |~ p] /\
+         (!q. q IN H ==> RTWN:(W->bool)#(W->W->bool)->bool |= q)
+         ==> RTWN:(W->bool)#(W->W->bool)->bool |= p`,
+  MESON_TAC[GEN_SUBS_CHAR_VALID; RTWN_SUBSET_CHAR_S4GRZ]);;
+
+(* ------------------------------------------------------------------------- *)
+(* Proof of soundness w.r.t. RATF.                                           *)
+(* ------------------------------------------------------------------------- *)
+
+let RTWN_VALID_IMPLIES_RATF_VALID = prove
+ (`!p. RTWN :(W->bool)#(W->W->bool)->bool |= p
+         ==> RATF:(W->bool)#(W->W->bool)->bool |= p`,
+  REWRITE_TAC[valid] THEN MESON_TAC[RATF_SUBSET_RTWN; SUBSET]);;
+
+let S4GRZ_RATF_VALID = prove
+ (`!p. [S4GRZ_AX . {} |~ p] ==> RATF:(W->bool)#(W->W->bool)->bool |= p`,
+  INTRO_TAC "!p; prove" THEN MATCH_MP_TAC RTWN_VALID_IMPLIES_RATF_VALID THEN
+  MATCH_MP_TAC S4GRZ_RTWN_VALID THEN EXISTS_TAC `{}:form->bool` THEN
+  ASM_MESON_TAC[NOT_IN_EMPTY]);;
+
+(* ------------------------------------------------------------------------- *)
+(* Proof of Consistency of S4GRZ.                                            *)
+(* ------------------------------------------------------------------------- *)
+
+let S4GRZ_CONSISTENT = prove
+ (`~ [S4GRZ_AX . {} |~  False]`,
+  REFUTE_THEN (MP_TAC o MATCH_MP(INST_TYPE[`:num`,`:W`] S4GRZ_RATF_VALID)) THEN
+  REWRITE_TAC[valid; holds; holds_in; FORALL_PAIR_THM; IN_RATF;
+    IN_FINITE_FRAME; REFLEXIVE; TRANSITIVE; ANTISYMMETRIC; NOT_FORALL_THM] THEN
+  MAP_EVERY EXISTS_TAC [`{0}`; `\x:num y:num. x = 0 /\ x = y`] THEN
+  REWRITE_TAC[NOT_INSERT_EMPTY; FINITE_SING; IN_SING] THEN MESON_TAC[]);;
+
+(* ------------------------------------------------------------------------- *)
+(* 4. Completeness Theorem                                                   *)
+(* ------------------------------------------------------------------------- *)
+
+(* ------------------------------------------------------------------------- *)
+(* S4GRZ standard worlds, frames and models.                                 *)
+(* ------------------------------------------------------------------------- *)
+
+let S4GRZ_STANDARD_WORLDS_DEF = new_definition
+  `S4GRZ_STANDARD_WORLDS p =
+   {w | MAXIMAL_CONSISTENT S4GRZ_AX p w /\
+        (!q. MEM q w  ==> (q SUBSENTENCE p \/
+                           ?C. Box C SUBFORMULA p /\
+                               (q = Box (C --> Box C) \/
+                                q = Not Box (C --> Box C))))}`;;
+
+let GEN_STANDARD_FRAME_DEF = new_definition
+  `GEN_STANDARD_FRAME S p =
+   APPR S INTER
+   {(W,R) | W = {w | MAXIMAL_CONSISTENT S p w /\
+            (!q. MEM q w ==> q SUBSENTENCE p)} /\
+            (!q w. Box q SUBFORMULA p /\ w IN W
+                   ==> (MEM (Box q) w <=> !x. R w x ==> MEM q x))}`;;
+
+let Q_REL_DEF = new_definition
+  `Q_REL p w x <=>
+    w IN S4GRZ_STANDARD_WORLDS p  /\
+    x IN S4GRZ_STANDARD_WORLDS p  /\
+    (!B. (B SUBSENTENCE p \/
+          (?C. Box C SUBFORMULA p /\
+           (Box B = Box(C --> Box C)))) ==>
+         (MEM (Box B) w ==> MEM (Box B) x))`;;
+
+let TRANSITIVE_Q_REL = prove
+ (`!p. TRANSITIVE (S4GRZ_STANDARD_WORLDS p) (Q_REL p)`,
+  REWRITE_TAC[TRANSITIVE; Q_REL_DEF] THEN MESON_TAC[]);;
+
+let S4GRZ_STANDARD_REL_DEF = new_definition
+  `S4GRZ_STANDARD_REL p w x <=>
+    w IN S4GRZ_STANDARD_WORLDS p  /\
+    x IN S4GRZ_STANDARD_WORLDS p  /\
+    Q_REL p w x /\ (Q_REL p x w ==> w = x)`;;
+
+(* ------------------------------------------------------------------------- *)
+(* The standard relation for S4GRZ is Reflexive, Antisymmetric               *)
+(* and Transitive.                                                           *)
+(* ------------------------------------------------------------------------- *)
+
+let S4GRZ_STANDARD_REL_PROP = prove
+ (`!p. REFLEXIVE (S4GRZ_STANDARD_WORLDS p) (S4GRZ_STANDARD_REL p) /\
+       ANTISYMMETRIC (S4GRZ_STANDARD_WORLDS p) (S4GRZ_STANDARD_REL p) /\
+       TRANSITIVE (S4GRZ_STANDARD_WORLDS p) (S4GRZ_STANDARD_REL p)`,
+  GEN_TAC THEN REPEAT CONJ_TAC THENL
+  [REWRITE_TAC[REFLEXIVE; S4GRZ_STANDARD_REL_DEF; Q_REL_DEF];
+   REWRITE_TAC[ANTISYMMETRIC; S4GRZ_STANDARD_REL_DEF] THEN
+   INTRO_TAC "!w w'; w w' (w w' (wQw' w'Qw_then)) (w w' (w'Qw wqw'_then))" THEN
+   FIRST_X_ASSUM MATCH_MP_TAC THEN ASM_REWRITE_TAC[];
+   REWRITE_TAC[TRANSITIVE; S4GRZ_STANDARD_REL_DEF] THEN
+   REPEAT GEN_TAC THEN STRIP_TAC THEN ASM_REWRITE_TAC[] THEN CONJ_TAC THENL
+   [ASM_MESON_TAC[TRANSITIVE_Q_REL; TRANSITIVE];
+    DISCH_TAC THEN
+    SUBGOAL_THEN `(w':(form)list) = w'' /\ w = w'` MP_TAC THENL
+    [CONJ_TAC THEN FIRST_X_ASSUM MATCH_MP_TAC THEN
+     ASM_MESON_TAC[TRANSITIVE_Q_REL; TRANSITIVE];
+     ASM_MESON_TAC[]]]]);;
+
+let S4GRZ_STANDARD_FRAME_DEF = new_definition
+ `S4GRZ_STANDARD_FRAME p =
+  {(W,R) | W = S4GRZ_STANDARD_WORLDS p /\
+           R = S4GRZ_STANDARD_REL p}`;;
+
+let S4GRZ_STANDARD_MODEL_DEF = new_definition
+ `S4GRZ_STANDARD_MODEL p (W,R) V <=>
+  (W,R) IN S4GRZ_STANDARD_FRAME p /\
+  (!a w. w IN W
+         ==> (V a w <=> MEM (Atom a) w /\ Atom a SUBFORMULA p))`;;
+
+(* ------------------------------------------------------------------------- *)
+(* Maximal Consistent Lemmas.                                                *)
+(* ------------------------------------------------------------------------- *)
+
+let EXTEND_MAXIMAL_CONSISTENT'' = prove
+ (`!S p X. CONSISTENT S X /\
+           (!q. MEM q X ==> q SUBSENTENCE p \/
+                            (?C. Box C SUBFORMULA p /\
+                                 (q = Box (C --> Box C) \/
+                                  q = Not Box (C --> Box C))))
+           ==> ?M. MAXIMAL_CONSISTENT S p M /\
+                   (!q. MEM q M ==> q SUBSENTENCE p  \/
+                            (?C. Box C SUBFORMULA p /\
+                                 (q = Box (C --> Box C) \/
+                                  q = Not Box (C --> Box C)))) /\
+                   X SUBLIST M`,
+  GEN_TAC THEN GEN_TAC THEN SUBGOAL_THEN
+    `!L X. CONSISTENT S X /\ NOREPETITION X /\
+           (!q. MEM q X ==> q SUBSENTENCE p \/
+                            (?C. Box C SUBFORMULA p /\
+                                 (q = Box (C --> Box C) \/
+                                  q = Not Box (C --> Box C)))) /\
+           (!q. MEM q L ==> q SUBFORMULA p) /\
+           (!q. q SUBFORMULA p ==> MEM q L \/ MEM q X \/ MEM (Not q) X)
+           ==> ?M. MAXIMAL_CONSISTENT S p M /\
+                   (!q. MEM q M ==> q SUBSENTENCE p \/
+                            (?C. Box C SUBFORMULA p /\
+                                 (q = Box (C --> Box C) \/
+                                  q = Not Box (C --> Box C)))) /\
+                   X SUBLIST M`
+    (LABEL_TAC "P") THENL
+  [ALL_TAC;
+   INTRO_TAC "![X']; cons' subf'" THEN
+   DESTRUCT_TAC "@X. uniq sub1 sub2"
+     (ISPEC `X':form list` EXISTS_NOREPETITION) THEN
+   DESTRUCT_TAC "@L'. uniq L'" (SPEC `p:form` SUBFORMULA_LIST) THEN
+   HYP_TAC "P: +" (SPECL[`L':form list`; `X:form list`]) THEN
+   ANTS_TAC THENL
+   [CONJ_TAC THENL [ASM_MESON_TAC[CONSISTENT_SUBLIST]; ALL_TAC] THEN
+    CONJ_TAC THENL [ASM_REWRITE_TAC[]; ALL_TAC] THEN
+    CONJ_TAC THENL [ASM_REWRITE_TAC[]; ALL_TAC] THEN
+    ASM_MESON_TAC[SUBLIST];
+    ALL_TAC] THEN
+   INTRO_TAC "@M. max sub" THEN EXISTS_TAC `M:form list` THEN
+   ASM_REWRITE_TAC[] THEN ASM_MESON_TAC[SUBLIST_TRANS]] THEN
+  LIST_INDUCT_TAC THENL
+  [REWRITE_TAC[MEM] THEN INTRO_TAC "!X; X uniq max subf" THEN
+   EXISTS_TAC `X:form list` THEN
+   ASM_REWRITE_TAC[SUBLIST_REFL; MAXIMAL_CONSISTENT];
+   ALL_TAC] THEN
+  POP_ASSUM (LABEL_TAC "hpind") THEN REWRITE_TAC[MEM] THEN
+  INTRO_TAC "!X; cons uniq qmem qmem' subf" THEN
+  LABEL_ASM_CASES_TAC "hmemX" `MEM (h:form) X` THENL
+  [REMOVE_THEN "hpind" (MP_TAC o SPEC `X:form list`) THEN
+   ASM_MESON_TAC[]; ALL_TAC] THEN
+  LABEL_ASM_CASES_TAC "nhmemX" `MEM (Not h) X` THENL
+  [REMOVE_THEN "hpind" (MP_TAC o SPEC `X:form list`) THEN
+   ASM_MESON_TAC[]; ALL_TAC] THEN
+  LABEL_ASM_CASES_TAC "consh" `CONSISTENT S (CONS (h:form) X)` THENL
+  [REMOVE_THEN "hpind" (MP_TAC o SPEC `CONS (h:form) X`) THEN
+   ANTS_TAC THENL
+   [ASM_REWRITE_TAC[NOREPETITION_CLAUSES; MEM] THEN
+    CONJ_TAC THENL [ALL_TAC; ASM_MESON_TAC[]] THEN
+    ASM_MESON_TAC[SUBLIST; SUBFORMULA_IMP_SUBSENTENCE];
+    ALL_TAC] THEN
+   INTRO_TAC "@M. max sub" THEN EXISTS_TAC `M:form list` THEN
+   ASM_REWRITE_TAC[] THEN REMOVE_THEN "sub" MP_TAC THEN
+   REWRITE_TAC[SUBLIST; MEM] THEN MESON_TAC[];
+   ALL_TAC] THEN
+  REMOVE_THEN "hpind" (MP_TAC o SPEC `CONS (Not h) X`) THEN ANTS_TAC THENL
+  [ASM_REWRITE_TAC[NOREPETITION_CLAUSES] THEN
+   CONJ_TAC THENL [ASM_MESON_TAC[CONSISTENT_EM]; ALL_TAC] THEN
+   REWRITE_TAC[MEM] THEN ASM_MESON_TAC[SUBLIST; SUBSENTENCE_RULES];
+   ALL_TAC] THEN
+  INTRO_TAC "@M. max sub" THEN EXISTS_TAC `M:form list` THEN
+  ASM_REWRITE_TAC[] THEN REMOVE_THEN "sub" MP_TAC THEN
+  REWRITE_TAC[SUBLIST; MEM] THEN MESON_TAC[]);;
+
+let NONEMPTY_MAXIMAL_CONSISTENT'' = prove
+ (`!S p. ~ [S . {} |~ p]
+         ==> ?M. MAXIMAL_CONSISTENT S p M /\
+                 MEM (Not p) M /\
+                 (!q. MEM q M ==> q SUBSENTENCE p \/
+                                   (?C. Box C SUBFORMULA p /\
+                                       (q = Box (C --> Box C) \/
+                                        q = Not Box (C --> Box C))))`,
+  INTRO_TAC "!S p; p" THEN
+  MP_TAC (SPECL [`S:form->bool`; `p:form`; `[Not p]`]
+    EXTEND_MAXIMAL_CONSISTENT'') THEN
+  ANTS_TAC THENL
+  [CONJ_TAC THENL
+   [REWRITE_TAC[CONSISTENT_SING] THEN ASM_MESON_TAC[MLK_DOUBLENEG_CL];
+    ALL_TAC] THEN
+   GEN_TAC THEN REWRITE_TAC[MEM] THEN
+   REPEAT STRIP_TAC THEN FIRST_X_ASSUM SUBST_VAR_TAC THEN
+   MESON_TAC[SUBFORMULA_IMP_NEG_SUBSENTENCE; SUBFORMULA_REFL];
+   ALL_TAC] THEN
+  STRIP_TAC THEN EXISTS_TAC `M:form list` THEN
+  ASM_REWRITE_TAC[] THEN ASM_MESON_TAC[SUBLIST; MEM]);;
+
+(* ------------------------------------------------------------------------- *)
+(* Truth Lemma.                                                              *)
+(* ------------------------------------------------------------------------- *)
+
+let S4GRZ_TRUTH_LEMMA = prove
+ (`!W R p V q. ~[S4GRZ_AX . {} |~ p] /\
+     q SUBFORMULA p /\ S4GRZ_STANDARD_MODEL p (W,R) V
+     ==> !w. w IN W  ==> (MEM q w <=> holds (W,R) V q w)`,
+  REPEAT GEN_TAC THEN
+  REWRITE_TAC[S4GRZ_STANDARD_MODEL_DEF; S4GRZ_STANDARD_FRAME_DEF;
+              S4GRZ_STANDARD_WORLDS_DEF; S4GRZ_STANDARD_REL_DEF;
+              IN_ELIM_THM; PAIR_EQ] THEN
+  INTRO_TAC "np q (@W' R'. (W' R') WW' RR' ) val" THEN
+  REMOVE_THEN "WW'" SUBST_VAR_TAC THEN
+  REMOVE_THEN "RR'" SUBST_VAR_TAC THEN
+  REMOVE_THEN "W'" SUBST_ALL_TAC THEN
+  REMOVE_THEN "R'" SUBST_ALL_TAC THEN
+  ASM_REWRITE_TAC[FORALL_IN_GSPEC] THEN
+  HYP_TAC "val" (REWRITE_RULE[FORALL_IN_GSPEC]) THEN
+  REMOVE_THEN "q" MP_TAC THEN
+  GEN_FORM_INDUCT_TAC `q:form` THEN REWRITE_TAC[holds]  THEN
+  INTRO_TAC "sub; !w; max_cons mem" THEN
+  TRY
+    (REMOVE_THEN "q1_hpind" MP_TAC THEN
+     MATCH_MP_TAC (MESON[] `P /\ (P /\ Q ==> R) ==> ((P ==> Q) ==> R)`) THEN
+     CONJ_TAC THENL
+     [ASM_MESON_TAC[SUBFORMULA_TRANS; SUBFORMULA_INVERSION; SUBFORMULA_REFL];
+      INTRO_TAC "sub1 +" THEN DISCH_THEN (MP_TAC o SPEC `w:form list`)] THEN
+     REMOVE_THEN "q2_hpind" MP_TAC THEN
+     MATCH_MP_TAC (MESON[] `P /\ (P /\ Q ==> R) ==> ((P ==> Q) ==> R)`) THEN
+     CONJ_TAC THENL
+     [ASM_MESON_TAC[SUBFORMULA_TRANS; SUBFORMULA_INVERSION; SUBFORMULA_REFL];
+      INTRO_TAC "sub2 +" THEN DISCH_THEN (MP_TAC o SPEC `w:form list`)] THEN
+     ASM_REWRITE_TAC[] THEN
+     INTRO_TAC "a; b" THEN
+     HYP_TAC "a" (GSYM) THEN ASM_REWRITE_TAC[] THEN
+     HYP_TAC "b" (GSYM) THEN ASM_REWRITE_TAC[] THEN
+     CLAIM_TAC "rmk"
+       `!q. q SUBFORMULA p
+            ==> (MEM q w <=> [S4GRZ_AX. {} |~ CONJLIST w --> q])` THENL
+     [ASM_MESON_TAC[MAXIMAL_CONSISTENT_SUBFORMULA_MEM_EQ_DERIVABLE];
+      ALL_TAC]) THENL
+  [
+   (* q = False *)
+   HYP_TAC "max_cons -> cons memq" (REWRITE_RULE[MAXIMAL_CONSISTENT]) THEN
+   ASM_MESON_TAC[FALSE_IMP_NOT_CONSISTENT]
+  ;
+   (* q = True *)
+   HYP_TAC "max_cons: (cons (norep mem))"
+         (REWRITE_RULE[MAXIMAL_CONSISTENT]) THEN
+   HYP_TAC "mem: t | nt" (C MATCH_MP (ASSUME `True SUBFORMULA p`)) THEN
+   ASM_REWRITE_TAC[] THEN REFUTE_THEN (K ALL_TAC) THEN
+   HYP MESON_TAC "cons nt" [NOT_CONSISTENT_1; MLK_DOUBLENEG; MLK_truth_th]
+  ;
+   (* q = Atom *)
+   ASM_SIMP_TAC[]
+  ;
+   (* q = Not a *)
+   REMOVE_THEN "q_hpind" MP_TAC THEN
+   MATCH_MP_TAC (MESON[] `P /\ (P /\ Q ==> R) ==> ((P ==> Q) ==> R)`) THEN
+   CONJ_TAC THENL
+   [ASM_MESON_TAC[SUBFORMULA_TRANS; SUBFORMULA_INVERSION; SUBFORMULA_REFL];
+   INTRO_TAC "sub1 q" THEN
+   EQ_TAC THENL
+   [REMOVE_THEN "q" (MP_TAC o SPEC `w: form list`) THEN
+    ANTS_TAC THEN ASM_REWRITE_TAC[] THEN
+    ASM_MESON_TAC[MAXIMAL_CONSISTENT_MEM_NOT];
+    REMOVE_THEN "q" (MP_TAC o SPEC `w: form list`) THEN
+    ANTS_TAC THEN ASM_REWRITE_TAC[] THEN
+    ASM_MESON_TAC[MAXIMAL_CONSISTENT_MEM_NOT]]]
+  ;
+   (* q = q1 && q2 *)
+   ASM_SIMP_TAC[] THEN
+   ASM_MESON_TAC[MAXIMAL_CONSISTENT_SUBFORMULA_MEM_EQ_DERIVABLE;
+    MLK_and_intro; MLK_and_left_th; MLK_and_right_th; MLK_imp_trans]
+  ;
+   (* q = q1 || q2 *)
+   EQ_TAC THENL
+   [INTRO_TAC "q1q2" THEN
+     CLAIM_TAC "wq1q2" `[S . {} |~ CONJLIST w --> q1 || q2]` THENL
+     [ASM_SIMP_TAC[CONJLIST_IMP_MEM]; ALL_TAC] THEN
+     CLAIM_TAC "hq1 | hq1" `MEM q1 w \/ MEM (Not q1) w` THENL
+     [ASM_MESON_TAC[MAXIMAL_CONSISTENT_MEM_CASES];
+      ASM_REWRITE_TAC[]; ALL_TAC] THEN
+     CLAIM_TAC "hq2 | hq2" `MEM q2 w \/ MEM (Not q2) w` THENL
+     [ASM_MESON_TAC[MAXIMAL_CONSISTENT_MEM_CASES];
+      ASM_REWRITE_TAC[]; REFUTE_THEN (K ALL_TAC)] THEN
+     SUBGOAL_THEN `~ ([S4GRZ_AX . {} |~ (CONJLIST w --> False)])` MP_TAC THENL
+     [REWRITE_TAC[GSYM MLK_not_def] THEN
+      HYP_TAC "max_cons : not norep sub" (REWRITE_RULE[MAXIMAL_CONSISTENT; CONSISTENT]) THEN
+      ASM_REWRITE_TAC[]; ALL_TAC] THEN
+     ASM_REWRITE_TAC[] THEN MATCH_MP_TAC MLK_frege THEN EXISTS_TAC `q1 || q2` THEN
+     ASM_SIMP_TAC[CONJLIST_IMP_MEM] THEN MATCH_MP_TAC MLK_imp_swap THEN
+     REWRITE_TAC[MLK_disj_imp] THEN CONJ_TAC THEN MATCH_MP_TAC MLK_imp_swap THEN
+     ASM_MESON_TAC[CONJLIST_IMP_MEM; MLK_axiom_not; MLK_iff_imp1; MLK_imp_trans];
+    ASM_MESON_TAC[MLK_or_left_th; MLK_or_right_th; MLK_imp_trans;
+                  MAXIMAL_CONSISTENT_SUBFORMULA_MEM_EQ_DERIVABLE]]
+  ;
+  (* q = q1 --> q2 *)
+  EQ_TAC THENL
+  [ASM_MESON_TAC[MLK_frege; CONJLIST_IMP_MEM;
+                 MAXIMAL_CONSISTENT_SUBFORMULA_MEM_EQ_DERIVABLE];
+   INTRO_TAC "imp" THEN
+    CLAIM_TAC "hq1 | hq1" `MEM q1 w \/ MEM (Not q1) w` THENL
+    [ASM_MESON_TAC[MAXIMAL_CONSISTENT_MEM_CASES];
+     ASM_MESON_TAC[CONJLIST_IMP_MEM; MLK_imp_swap; MLK_add_assum;
+     MAXIMAL_CONSISTENT_SUBFORMULA_MEM_EQ_DERIVABLE];
+     ALL_TAC] THEN
+    MP_TAC (SPECL[`S4GRZ_AX`; `p:form`; `w:form list`; `q1 --> q2`]
+            MAXIMAL_CONSISTENT_SUBFORMULA_MEM_EQ_DERIVABLE) THEN
+    ASM_REWRITE_TAC[] THEN DISCH_TAC THEN ASM_REWRITE_TAC[] THEN
+    MATCH_MP_TAC MLK_shunt THEN MATCH_MP_TAC MLK_imp_trans THEN
+          EXISTS_TAC `q1 && Not q1` THEN CONJ_TAC THENL
+          [ALL_TAC; MESON_TAC[MLK_nc_th; MLK_imp_trans; MLK_ex_falso_th]] THEN
+          MATCH_MP_TAC MLK_and_intro THEN REWRITE_TAC[MLK_and_right_th] THEN
+          ASM_MESON_TAC[CONJLIST_IMP_MEM; MLK_imp_trans; MLK_and_left_th]]
+  ;
+   (* q = q1 <-> q2 *)
+   ASM_SIMP_TAC[] THEN REMOVE_THEN "sub" (K ALL_TAC) THEN EQ_TAC THENL
+   [MESON_TAC[MLK_frege; MLK_add_assum; MLK_modusponens_th;
+           MLK_axiom_iffimp1; MLK_axiom_iffimp2];
+   ALL_TAC] THEN
+   INTRO_TAC "iff" THEN MATCH_MP_TAC MLK_imp_trans THEN
+   EXISTS_TAC `(q1 --> q2) && (q2 --> q1)` THEN CONJ_TAC THENL
+   [MATCH_MP_TAC MLK_and_intro; MESON_TAC[MLK_iff_def_th; MLK_iff_imp2]] THEN
+   CLAIM_TAC "rmk'"
+     `!q. q SUBFORMULA p
+         ==> (MEM (Not q) w <=> [S4GRZ_AX. {} |~ CONJLIST w --> Not q])` THENL
+   [ASM_MESON_TAC[MAXIMAL_CONSISTENT_SUBFORMULA_MEM_NEG_EQ_DERIVABLE];
+    ALL_TAC] THEN
+   CLAIM_TAC "hq1 | hq1"
+    `[S4GRZ_AX. {} |~ (CONJLIST w --> q1)] \/
+     [S4GRZ_AX. {} |~ CONJLIST w --> Not q1]` THENL
+   [ASM_MESON_TAC[MAXIMAL_CONSISTENT_MEM_CASES];
+    ASM_MESON_TAC[MLK_imp_swap; MLK_add_assum];
+    ALL_TAC] THEN
+  CLAIM_TAC "hq2 | hq2"
+     `[S4GRZ_AX. {} |~ (CONJLIST w --> q2)] \/
+     [S4GRZ_AX. {} |~ (CONJLIST w --> Not q2)]` THENL
+   [ASM_MESON_TAC[MAXIMAL_CONSISTENT_MEM_CASES];
+    ASM_MESON_TAC[MLK_imp_swap; MLK_add_assum];
+    ALL_TAC] THEN
+   ASM_MESON_TAC[MLK_nc_th; MLK_imp_trans; MLK_and_intro;
+                  MLK_ex_falso_th; MLK_imp_swap; MLK_shunt]
+  ;
+  (* q = Box q1*)
+  CLAIM_TAC "suba" `q SUBFORMULA p` THENL
+  [MATCH_MP_TAC SUBFORMULA_TRANS THEN EXISTS_TAC `Box q` THEN
+   ASM_REWRITE_TAC[SUBFORMULA_INVERSION; SUBFORMULA_REFL];
+   ALL_TAC] THEN
+  ASM_CASES_TAC `MEM (Box q)  (w:form list)` THENL
+  [ASM_REWRITE_TAC[IN_ELIM_THM] THEN
+    INTRO_TAC "!w'; (max_cons_w mem_w') ww'" THEN
+    CLAIM_TAC "memw'" `MEM q  (w':form list)` THENL
+    [MATCH_MP_TAC MAXIMAL_CONSISTENT_LEMMA THEN
+     EXISTS_TAC `S4GRZ_AX` THEN
+     EXISTS_TAC `p:form` THEN
+     EXISTS_TAC `[Box q]` THEN
+     ASM_REWRITE_TAC[MEM] THEN
+     CONJ_TAC THENL
+     [INTRO_TAC "!q'; eq" THEN ASM_REWRITE_TAC[] THEN
+       HYP_TAC "ww': w w' (w w' wQw') w'Qw_then"
+         (REWRITE_RULE[S4GRZ_STANDARD_REL_DEF; Q_REL_DEF; SUBSENTENCE_CASES]) THEN
+       ASM_MESON_TAC[];
+      ASM_MESON_TAC[CONJLIST; GRZ_PROVES_T; T_SCHEMA_DEF; GRZ_EQ_S4GRZ]]; ALL_TAC] THEN
+    HYP_TAC "q_hpind" (C MATCH_MP (ASSUME `q SUBFORMULA p`)) THEN
+    HYP_TAC "q_hpind: +" (SPEC `w':form list`) THEN
+    ANTS_TAC THENL [ASM_REWRITE_TAC[]; ALL_TAC] THEN
+    DISCH_THEN (SUBST1_TAC o GSYM) THEN ASM_REWRITE_TAC[];
+   ALL_TAC] THEN
+   ASM_REWRITE_TAC[IN_ELIM_THM; NOT_FORALL_THM; NOT_IMP] THEN
+   CLAIM_TAC "NotBox_mem" `MEM (Not Box q) (w:form list)` THENL
+   [ASM_MESON_TAC[MAXIMAL_CONSISTENT_MEM_NOT]; ALL_TAC] THEN
+   ASM_CASES_TAC `~(MEM q (w:form list))` THENL
+   [EXISTS_TAC `w:form list` THEN
+    ASM_REWRITE_TAC[] THEN CONJ_TAC THENL
+    [MP_TAC (SPEC `p:form` S4GRZ_STANDARD_REL_PROP) THEN
+      ASM_REWRITE_TAC[REFLEXIVE] THEN
+      INTRO_TAC "refl antsym trans" THEN
+      FIRST_X_ASSUM MATCH_MP_TAC THEN
+      ASM_REWRITE_TAC[S4GRZ_STANDARD_WORLDS_DEF; IN_ELIM_THM; S4GRZ_STANDARD_REL_PROP];
+     HYP_TAC "q_hpind" (C MATCH_MP (ASSUME `q SUBFORMULA p`)) THEN
+     HYP_TAC "q_hpind: +" (SPEC `w:form list`) THEN
+     ANTS_TAC THENL [ASM_REWRITE_TAC[]; ALL_TAC] THEN
+     DISCH_THEN (SUBST1_TAC o GSYM) THEN ASM_REWRITE_TAC[]]; ALL_TAC] THEN
+  FIRST_ASSUM MP_TAC THEN REWRITE_TAC[] THEN INTRO_TAC "q_mem" THEN
+  CLAIM_TAC "Box_imp_Box_not_mem" `~(MEM (Box (q --> Box q)) (w:form list))` THENL
+  [REFUTE_THEN MP_TAC THEN INTRO_TAC "Box_imp_Box_mem" THEN
+   SUBGOAL_THEN `MEM (Box q) (w:form list)` MP_TAC THENL
+   [MATCH_MP_TAC MAXIMAL_CONSISTENT_LEMMA THEN
+    EXISTS_TAC `S4GRZ_AX` THEN
+    EXISTS_TAC `p:form` THEN
+    EXISTS_TAC `[Box (q --> Box q); q]` THEN
+    ASM_REWRITE_TAC[MEM] THEN
+    CONJ_TAC THENL
+    [REPEAT STRIP_TAC THEN ASM_REWRITE_TAC[] THEN ASM_REWRITE_TAC[];
+     ASM_REWRITE_TAC[CONJLIST; NOT_CONS_NIL] THEN MATCH_MP_TAC S4GRZ_prove_S4 THEN
+      HOLMS_TAC] THEN
+    ASM_REWRITE_TAC[]; ALL_TAC] THEN
+    ASM_MESON_TAC[]; ALL_TAC] THEN
+   CLAIM_TAC "consistent_X"
+             `CONSISTENT S4GRZ_AX
+               (CONS (Not q)
+                     (APPEND (FLATMAP (\x. match x with Box c -> [Box c] | _ -> []) w)
+                             [Box (q --> Box q)]))` THENL
+   [REFUTE_THEN MP_TAC THEN
+    INTRO_TAC "non_cons" THEN
+    HYP_TAC "non_cons" (REWRITE_RULE[CONSISTENT; CONJLIST; APPEND_EQ_NIL; NOT_CONS_NIL]) THEN
+    CLAIM_TAC "1" `[S4GRZ_AX . {} |~ Not (Not q &&
+                                          (CONJLIST (FLATMAP (\x. match x with Box c -> [Box c] | _ -> []) w) &&
+                                           CONJLIST [Box (q --> Box q)]))]` THENL
+    [MATCH_MP_TAC MLK_not_subst_th THEN
+     EXISTS_TAC `Not q &&
+                 CONJLIST (APPEND (FLATMAP (\x. match x with Box c -> [Box c] | _ -> []) w)
+                                   [Box (q --> Box q)])` THEN
+     ASM_REWRITE_TAC[] THEN
+     MATCH_MP_TAC MLK_and_subst_th THEN
+     ASM_REWRITE_TAC[MLK_iff_refl_th; CONJLIST_APPEND; CONJLIST]; ALL_TAC] THEN
+    HYP_TAC "1" (REWRITE_RULE[CONJLIST]) THEN
+    CLAIM_TAC "2" `[S4GRZ_AX . {} |~ Box Box CONJLIST (FLATMAP (\x. match x with Box c -> [ Box c] | _ -> []) w) --> Box q]` THENL
+    [MATCH_MP_TAC MLK_imp_box THEN
+     MATCH_MP_TAC MLK_imp_trans THEN
+     EXISTS_TAC `Box (Box (q --> Box q) --> q)` THEN
+     ASM_REWRITE_TAC[S4GRZ_AX_GRZ] THEN
+     MATCH_MP_TAC MLK_imp_box THEN
+     MATCH_MP_TAC MLK_iff_mp THEN
+     EXISTS_TAC `Not (Not q &&
+                      CONJLIST (FLATMAP (\x. match x with Box c -> [Box c] | _ -> []) w) &&
+                                Box (q --> Box q))` THEN
+     CONJ_TAC THENL
+     [MATCH_MP_TAC S4GRZ_prove_S4 THEN
+       CLAIM_TAC "s4" `!a b c. [S4_AX . {} |~ Not (Not a && b && c) <-> b --> (c --> a)]` THENL
+       [HOLMS_TAC; ALL_TAC] THEN
+       ASM_MESON_TAC[];
+      ASM_REWRITE_TAC[]]; ALL_TAC] THEN
+    CLAIM_TAC "3" `[S4GRZ_AX . {} |~ CONJLIST (FLATMAP (\x. match x with Box c -> [ Box c] | _ -> []) w) --> Box q]` THENL
+    [MATCH_MP_TAC MLK_imp_trans THEN
+     EXISTS_TAC `Box Box CONJLIST (FLATMAP (\x. match x with Box c -> [Box c] | _ -> []) w)` THEN
+     ASM_REWRITE_TAC[] THEN
+     MATCH_MP_TAC MLK_imp_mp_subst THEN
+     EXISTS_TAC `CONJLIST (MAP (Box)
+                               (FLATMAP (\x. match x with Box c -> [c] | _ -> [])w))` THEN
+     EXISTS_TAC `Box Box CONJLIST (MAP (Box)
+                              (FLATMAP (\x. match x with Box c -> [c] | _ -> []) w))` THEN
+     REPEAT CONJ_TAC THENL
+     [REWRITE_TAC[MLK_iff_sym] THEN
+       MATCH_ACCEPT_TAC (CONJLIST_FLATMAP_DOT_BOX_LEMMA_3);
+      MATCH_MP_TAC MLK_box_subst THEN
+       MATCH_MP_TAC MLK_box_subst THEN
+       REWRITE_TAC[MLK_iff_sym] THEN
+       MATCH_ACCEPT_TAC (CONJLIST_FLATMAP_DOT_BOX_LEMMA_3);
+      MATCH_MP_TAC MLK_imp_mp_subst]
+     THEN
+     EXISTS_TAC `Box CONJLIST
+                      (FLATMAP (\x. match x with Box c -> [c] | _ -> []) w)` THEN
+     EXISTS_TAC `Box Box Box CONJLIST
+                              (FLATMAP (\x. match x with Box c -> [c] | _ -> []) w)`THEN
+     REPEAT CONJ_TAC THENL
+     [GEN_REWRITE_TAC I [MLK_iff_sym] THEN
+       ASM_REWRITE_TAC[CONJLIST_MAP_BOX];
+      GEN_REWRITE_TAC I [MLK_iff_sym] THEN
+       MATCH_MP_TAC MLK_box_subst THEN
+       MATCH_MP_TAC MLK_box_subst THEN
+       ASM_REWRITE_TAC[CONJLIST_MAP_BOX];
+      MATCH_MP_TAC S4GRZ_prove_S4 THEN
+       CLAIM_TAC "s4" `!q. [S4_AX . {} |~  Box q --> Box Box Box q]` THENL
+       [HOLMS_TAC; ALL_TAC] THEN
+      ASM_MESON_TAC[]]; ALL_TAC] THEN
+    SUBGOAL_THEN `MEM (Box q) w` MP_TAC THENL
+    [MATCH_MP_TAC MAXIMAL_CONSISTENT_LEMMA THEN
+     EXISTS_TAC `S4GRZ_AX` THEN
+     EXISTS_TAC `p:form` THEN
+     EXISTS_TAC `FLATMAP (\x. match x with Box c -> [Box c] | _ -> []) w` THEN
+     ASM_MESON_TAC[MEM_FLATMAP_LEMMA_2]; ALL_TAC] THEN
+    ASM_REWRITE_TAC[]; ALL_TAC]  THEN
+   CLAIM_TAC "@x. max_cons_x mem_x subl"
+             `?x. MAXIMAL_CONSISTENT S4GRZ_AX p x /\
+                  (!q. MEM q x ==> q SUBSENTENCE p \/
+                                   (?C. Box C SUBFORMULA p /\
+                                       (q = Box (C --> Box C) \/
+                                         q = Not Box (C --> Box C)))) /\
+                  (CONS (Not q) (APPEND (FLATMAP (\x. match x with Box c -> [Box c] | _ -> []) w)
+                                        [Box (q --> Box q)]))
+                   SUBLIST x` THENL
+   [MATCH_MP_TAC (EXTEND_MAXIMAL_CONSISTENT'') THEN
+    ASM_REWRITE_TAC[MEM; MEM_APPEND; CONSISTENT] THEN
+    REPEAT STRIP_TAC THENL
+    [DISJ1_TAC THEN
+      ASM_REWRITE_TAC[SUBSENTENCE_CASES] THEN
+      DISJ2_TAC THEN
+      EXISTS_TAC `q:form` THEN
+      ASM_REWRITE_TAC[];
+     CLAIM_TAC "@r. Box mem_w" `?r. q' = Box r /\ MEM q' w` THENL
+      [ASM_MESON_TAC[MEM_FLATMAP_LEMMA_2]; ALL_TAC] THEN
+      ASM_MESON_TAC[];
+     ASM_MESON_TAC[]]; ALL_TAC] THEN
+   EXISTS_TAC `x: form list` THEN
+   ASM_REWRITE_TAC[] THEN
+   CONJ_TAC THENL
+   [ASM_REWRITE_TAC[S4GRZ_STANDARD_REL_DEF; S4GRZ_STANDARD_WORLDS_DEF; IN_ELIM_THM] THEN
+     CONJ_TAC THENL
+     [ASM_REWRITE_TAC[Q_REL_DEF; S4GRZ_STANDARD_WORLDS_DEF; IN_ELIM_THM] THEN
+       REPEAT STRIP_TAC THENL
+      [SUBGOAL_THEN `MEM (Box B) (FLATMAP (\x. match x with Box c -> [Box c] | _ -> []) w)` MP_TAC THENL
+         [ASM_REWRITE_TAC[MEM_FLATMAP_LEMMA_2] THEN
+          ASM_MESON_TAC[]; ALL_TAC] THEN
+         HYP_TAC "subl" (REWRITE_RULE[SUBLIST; MEM; MEM_APPEND]) THEN
+         ASM_MESON_TAC[];
+        ASM_REWRITE_TAC[] THEN
+         SUBGOAL_THEN `MEM (Box B) (FLATMAP (\x. match x with Box c -> [Box c] | _ -> []) w)` MP_TAC THENL
+         [ASM_REWRITE_TAC[MEM_FLATMAP_LEMMA_2] THEN ASM_MESON_TAC[]; ALL_TAC] THEN
+         HYP_TAC "subl" (REWRITE_RULE[SUBLIST; MEM; MEM_APPEND]) THEN ASM_MESON_TAC[]];
+      GEN_REWRITE_TAC I [GSYM CONTRAPOS_THM] THEN
+       DISCH_TAC THEN
+       ASM_REWRITE_TAC[Q_REL_DEF; DE_MORGAN_THM; TAUT `(~p \/ ~q \/ ~r) <=> (p /\ q ==> ~ r)`;
+                               NOT_FORALL_THM; NOT_IMP] THEN
+       DISJ2_TAC THEN DISJ2_TAC THEN
+       EXISTS_TAC `q --> Box q` THEN
+       CONJ_TAC THENL
+       [DISJ2_TAC THEN EXISTS_TAC `q:form` THEN
+         ASM_REWRITE_TAC[];
+        REWRITE_TAC[TAUT `~(p <=> q) <=> (p /\ ~q) \/ (~p /\ q)`] THEN
+        CONJ_TAC THENL
+        [HYP_TAC "subl" (REWRITE_RULE[SUBLIST; MEM; MEM_APPEND]) THEN
+          ASM_MESON_TAC[];
+         ASM_REWRITE_TAC[]]]];
+   SUBGOAL_THEN `~(MEM (q:form) x)` MP_TAC THENL
+   [SUBGOAL_THEN `MEM (Not q) x` MP_TAC THENL
+    [HYP_TAC "subl" (REWRITE_RULE[SUBLIST; MEM; MEM_APPEND]) THEN
+     ASM_MESON_TAC[]; ALL_TAC] THEN
+    ASM_MESON_TAC[MAXIMAL_CONSISTENT_MEM_NOT]; ALL_TAC] THEN
+   HYP_TAC "q_hpind -> +" (REWRITE_RULE[]) THEN
+   MATCH_MP_TAC (MESON[] `P /\ (Q ==> R) ==> ((P ==> Q) ==> R)`) THEN
+   ASM_REWRITE_TAC[] THEN
+   INTRO_TAC "a" THEN
+   HYP_TAC "a" (SPEC `x: form list`) THEN
+   ASM_MESON_TAC[]]]);;
+
+(* ------------------------------------------------------------------------- *)
+(* Proof of Completeness w.r.t. RATF.                                        *)
+(* ------------------------------------------------------------------------- *)
+
+let S4GRZ_COMPLETENESS_THM = prove
+ (`!p. RATF:(form list->bool)#(form list->form list->bool)->bool |= p
+       ==> [S4GRZ_AX . {} |~ p]`,
+  GEN_TAC THEN GEN_REWRITE_TAC I [GSYM CONTRAPOS_THM] THEN
+  INTRO_TAC "p_not_theor" THEN
+  REWRITE_TAC[valid; NOT_FORALL_THM] THEN
+  EXISTS_TAC `(S4GRZ_STANDARD_WORLDS p,
+                S4GRZ_STANDARD_REL p)` THEN
+  REWRITE_TAC[NOT_IMP] THEN CONJ_TAC THENL
+  [ASM_REWRITE_TAC[IN_RATF; S4GRZ_STANDARD_REL_PROP; IN_FINITE_FRAME;
+                   S4GRZ_STANDARD_WORLDS_DEF] THEN
+  CONJ_TAC THENL (* non empty *)
+  [REWRITE_TAC[GSYM MEMBER_NOT_EMPTY; IN_ELIM_THM] THEN
+    SUBGOAL_THEN `(?M. MAXIMAL_CONSISTENT S4GRZ_AX p M /\
+                          MEM (Not p) M /\
+                          (!q. MEM q M ==>
+                               q SUBSENTENCE p \/
+                               (?C. Box C SUBFORMULA p /\
+                                (q = Box (C --> Box C) \/
+                                 q = Not Box (C --> Box C)))))`
+                   MP_TAC THENL
+    [MATCH_MP_TAC NONEMPTY_MAXIMAL_CONSISTENT'' THEN
+    ASM_MESON_TAC[]; ALL_TAC] THEN
+    INTRO_TAC "@M. max mem sub" THEN
+    EXISTS_TAC`M:form list` THEN
+    ASM_REWRITE_TAC[];
+   CONJ_TAC THENL (* well define *)
+   [REWRITE_TAC[S4GRZ_STANDARD_REL_DEF; S4GRZ_STANDARD_WORLDS_DEF] THEN
+   INTRO_TAC "!x y; x y Q" THEN ASM_REWRITE_TAC[];
+    (* finite *)
+  MATCH_MP_TAC FINITE_SUBSET THEN
+   EXISTS_TAC `{l | NOREPETITION l /\
+                    !q. MEM q l ==>
+                        q IN {q | q SUBSENTENCE p \/
+                                  (?C. Box C SUBFORMULA p /\
+                                       (q = Box (C --> Box C) \/
+                                        q = Not Box (C --> Box C)))}}` THEN
+   CONJ_TAC THENL [ALL_TAC; ASM SET_TAC[MAXIMAL_CONSISTENT]] THEN
+   MATCH_MP_TAC FINITE_NOREPETITION THEN
+   POP_ASSUM_LIST (K ALL_TAC) THEN
+   SUBGOAL_THEN `{q | q SUBSENTENCE p  \/
+                      (?C. Box C SUBFORMULA p /\
+                           (q = Box (C --> Box C) \/
+                            q = Not Box (C --> Box C)))} =
+                 {q | q SUBFORMULA p} UNION
+                 IMAGE (Not) {q | q SUBFORMULA p} UNION
+                 {q | ?C. (C IN {q | Box q IN {q | q SUBFORMULA p}}) /\
+                                     q = Box (C --> Box C)} UNION
+                 IMAGE (Not) {q | ? C. (C  IN {q | Box q IN {q | q SUBFORMULA p}}) /\
+                                      q = Box (C --> Box C)}`
+     SUBST1_TAC THENL
+  [REWRITE_TAC[GSYM SUBSET_ANTISYM_EQ; SUBSET; FORALL_IN_UNION;
+                FORALL_IN_GSPEC; FORALL_IN_IMAGE] THEN
+    REWRITE_TAC[IN_UNION; IN_ELIM_THM; SUBSENTENCE_RULES] THEN
+    REPEAT CONJ_TAC THENL
+    [GEN_TAC THEN REWRITE_TAC[SUBSENTENCE_CASES] THEN
+     STRIP_TAC THENL
+     [ASM SET_TAC[];
+      ASM SET_TAC[];
+      ASM SET_TAC[];
+      ASM SET_TAC[]];
+    MESON_TAC[SUBSENTENCE_CASES];
+    MESON_TAC[SUBSENTENCE_CASES];
+    MESON_TAC[SUBSENTENCE_CASES];
+    MESON_TAC[SUBSENTENCE_CASES]];
+   REWRITE_TAC[FINITE_UNION; FINITE_SUBFORMULA] THEN
+    CONJ_TAC THENL
+    [MATCH_MP_TAC FINITE_IMAGE THEN REWRITE_TAC[FINITE_SUBFORMULA];
+     CONJ_TAC THENL
+     [MATCH_MP_TAC     FINITE_IMAGE_EXPAND     THEN
+        MATCH_MP_TAC FINITE_SUBSET THEN
+        EXISTS_TAC `{q | q SUBFORMULA p}` THEN
+        REWRITE_TAC[FINITE_SUBFORMULA; SUBSET; IN_ELIM_THM] THEN
+        INTRO_TAC "!x; Box_sub" THEN
+        MATCH_MP_TAC SUBFORMULA_TRANS THEN
+        EXISTS_TAC `Box x` THEN
+        ASM_REWRITE_TAC[] THEN
+        ONCE_REWRITE_TAC[SUBFORMULA_CASES_L] THEN
+        DISJ2_TAC THEN EXISTS_TAC `x: form` THEN
+        ASM_REWRITE_TAC[SUBFORMULA_REFL; IN_MINOR_CASES];
+        MATCH_MP_TAC FINITE_IMAGE THEN
+        MATCH_MP_TAC FINITE_IMAGE_EXPAND THEN
+        MATCH_MP_TAC FINITE_SUBSET THEN
+        EXISTS_TAC `{q | q SUBFORMULA p}` THEN
+        REWRITE_TAC[FINITE_SUBFORMULA; SUBSET; IN_ELIM_THM] THEN
+        INTRO_TAC "!x; Box_sub" THEN
+        MATCH_MP_TAC SUBFORMULA_TRANS THEN
+        EXISTS_TAC `Box x` THEN
+        ASM_REWRITE_TAC[] THEN
+        ONCE_REWRITE_TAC[SUBFORMULA_CASES_L] THEN
+        DISJ2_TAC THEN EXISTS_TAC `x: form` THEN
+      ASM_REWRITE_TAC[SUBFORMULA_REFL; IN_MINOR_CASES]]]]]];
+  ASM_REWRITE_TAC[holds_in; NOT_FORALL_THM; NOT_IMP] THEN
+   EXISTS_TAC `\a M. Atom a SUBFORMULA p /\ MEM (Atom a) M` THEN
+   DESTRUCT_TAC "@M. max mem subf"
+      (MATCH_MP NONEMPTY_MAXIMAL_CONSISTENT'' (ASSUME `~ [S4GRZ_AX . {} |~ p]`)) THEN
+   EXISTS_TAC `M:form list` THEN ASM_REWRITE_TAC[] THEN
+   CONJ_TAC THENL
+   [ASM_REWRITE_TAC[S4GRZ_STANDARD_WORLDS_DEF; IN_ELIM_THM];
+   MP_TAC (ISPECL [`S4GRZ_STANDARD_WORLDS p`;
+                   `S4GRZ_STANDARD_REL p`;
+                   `p:form`;
+                   `(\a M. Atom a SUBFORMULA p /\ MEM (Atom a) M)`;
+                   `p:form`] S4GRZ_TRUTH_LEMMA) THEN
+   ANTS_TAC THENL
+   [ASM_REWRITE_TAC[SUBFORMULA_REFL] THEN
+    ASM_REWRITE_TAC[S4GRZ_STANDARD_MODEL_DEF; S4GRZ_STANDARD_FRAME_DEF;
+                   IN_ELIM_THM] THEN
+    ASM_MESON_TAC[];
+    DISCH_THEN (MP_TAC o SPEC `M:form list`) THEN
+    ANTS_TAC THENL
+    [ASM_REWRITE_TAC[S4GRZ_STANDARD_WORLDS_DEF; IN_ELIM_THM];
+     DISCH_THEN (SUBST1_TAC o GSYM) THEN
+     ASM_MESON_TAC[MAXIMAL_CONSISTENT; CONSISTENT_NC]]]]]);;
+
+(* ------------------------------------------------------------------------- *)
+(* Completeness Theorem for S4Grz on a generic (infinite) domain.            *)
+(* ------------------------------------------------------------------------- *)
+
+let S4GRZ_COMPLETENESS_THM_GEN = prove
+ (`!p. INFINITE (:A) /\ RATF:(A->bool)#(A->A->bool)->bool |= p
+       ==> [S4GRZ_AX . {} |~ p]`,
+  SUBGOAL_THEN
+    `INFINITE (:A)
+     ==> !p. RATF:(A->bool)#(A->A->bool)->bool |= p
+             ==> RATF:(form list->bool)#(form list->form list->bool)->bool |= p`
+    (fun th -> MESON_TAC[th; S4GRZ_COMPLETENESS_THM]) THEN
+  INTRO_TAC "A" THEN MATCH_MP_TAC BISIMILAR_VALID THEN
+  REWRITE_TAC[IN_RATF] THEN
+  REPEAT GEN_TAC THEN INTRO_TAC "(finite1 refl trans anti) w1" THEN
+  CLAIM_TAC "@f. inj" `?f:form list->A. (!x y. f x = f y ==> x = y)` THENL
+  [SUBGOAL_THEN `(:form list) <=_c (:A)` MP_TAC THENL
+   [TRANS_TAC CARD_LE_TRANS `(:num)` THEN
+    ASM_REWRITE_TAC[GSYM INFINITE_CARD_LE; GSYM COUNTABLE_ALT] THEN
+    ASM_SIMP_TAC[COUNTABLE_LIST; COUNTABLE_FORM];
+    REWRITE_TAC[le_c; IN_UNIV]];
+   ALL_TAC] THEN
+  MAP_EVERY EXISTS_TAC
+    [`IMAGE (f:form list->A) W1`;
+     `\x y:A. ?a b:form list.
+        a IN W1 /\ b IN W1 /\ x = f a /\ y = f b /\ R1 a b`;
+     `\a:string w:A. ?x:form list. w = f x /\ V1 a x`;
+     `f (w1:form list):A`] THEN
+   CONJ_TAC THENL
+  [REWRITE_TAC[IN_FINITE_FRAME] THEN
+   CONJ_TAC THENL
+   [CONJ_TAC THENL [HYP SET_TAC "w1" []; ALL_TAC] THEN
+   CONJ_TAC THENL [SET_TAC[]; ALL_TAC] THEN
+   ASM_MESON_TAC[IN_FINITE_FRAME; FINITE_IMAGE]; ALL_TAC] THEN
+   CONJ_TAC THENL
+   [REWRITE_TAC[REFLEXIVE; FORALL_IN_IMAGE] THEN
+    HYP_TAC "refl" (REWRITE_RULE[REFLEXIVE]) THEN
+    HYP MESON_TAC "refl inj" [];
+    ALL_TAC] THEN
+    CONJ_TAC THENL
+   [REWRITE_TAC[TRANSITIVE; FORALL_IN_IMAGE] THEN
+    HYP_TAC "trans" (REWRITE_RULE[TRANSITIVE]) THEN
+    HYP MESON_TAC "trans inj" [];
+    ALL_TAC] THEN
+    REWRITE_TAC[ANTISYMMETRIC; FORALL_IN_IMAGE] THEN
+    HYP_TAC "anti" (REWRITE_RULE[ANTISYMMETRIC]) THEN
+    HYP MESON_TAC "anti inj" []; ALL_TAC] THEN
+    REWRITE_TAC[BISIMILAR] THEN
+    EXISTS_TAC `\w1:form list w2:A. w1 IN W1 /\ w2 = f w1` THEN
+    ASM_REWRITE_TAC[BISIMIMULATION] THEN REMOVE_THEN "w1" (K ALL_TAC) THEN
+    REPEAT GEN_TAC THEN STRIP_TAC THEN FIRST_X_ASSUM SUBST_VAR_TAC THEN
+    ASM_SIMP_TAC[FUN_IN_IMAGE] THEN
+    CONJ_TAC THENL [HYP MESON_TAC "inj" []; ALL_TAC] THEN
+    CONJ_TAC THENL
+    [REPEAT STRIP_TAC THEN REWRITE_TAC[EXISTS_IN_IMAGE] THEN
+    ASM_MESON_TAC[IN_FINITE_FRAME];
+    ALL_TAC] THEN
+    ASM_MESON_TAC[]);;
+
+(* ------------------------------------------------------------------------- *)
+(* 5. Adequacy Theorem                                                       *)
+(* ------------------------------------------------------------------------- *)
+
+(* ------------------------------------------------------------------------- *)
+(* Semantical Adequacy of Grz.                                               *)
+(* ------------------------------------------------------------------------- *)
+
+let GRZ_ADEQ_THM = prove
+ (`!p. RATF:(form list->bool)#(form list->form list->bool)->bool |= p
+       <=> [GRZ_AX . {} |~ p]`,
+  GEN_TAC THEN EQ_TAC THENL
+   [INTRO_TAC "RATF" THEN REWRITE_TAC [GRZ_EQ_S4GRZ] THEN
+   ASM_MESON_TAC [S4GRZ_COMPLETENESS_THM]; ALL_TAC] THEN
+   INTRO_TAC "Grz" THEN MATCH_MP_TAC S4GRZ_RATF_VALID THEN
+   ASM_MESON_TAC [GRZ_EQ_S4GRZ]);;
+
+let GRZ_ADEQ_THM_num = prove
+ (`!p. RATF:(num->bool)#(num->num->bool)->bool |= p
+       <=> [GRZ_AX . {} |~ p]`,
+  GEN_TAC THEN EQ_TAC THENL
+   [INTRO_TAC "RATF" THEN REWRITE_TAC [GRZ_EQ_S4GRZ] THEN
+   MATCH_MP_TAC (INST_TYPE [`:num`,`:A`] S4GRZ_COMPLETENESS_THM_GEN) THEN
+   ASM_REWRITE_TAC[INFINITE_CARD_LE] THEN
+   MATCH_MP_TAC CARD_EQ_IMP_LE THEN
+   MATCH_ACCEPT_TAC CARD_EQ_REFL; ALL_TAC] THEN
+   INTRO_TAC "Grz" THEN MATCH_MP_TAC S4GRZ_RATF_VALID THEN
+   ASM_MESON_TAC [GRZ_EQ_S4GRZ]);;
+
+(* ------------------------------------------------------------------------- *)
+(* 6. Translation for Grz to GL.                                             *)
+(* ------------------------------------------------------------------------- *)
+
+let R_PLUS_DEF = new_definition
+  `R_PLUS (W:W->bool) (R:W->W->bool) w x <=>
+     ((R w x) \/ (w IN W /\ w = x))`;;
+
+let R_MIN_DEF = new_definition
+  `R_MIN (W:W->bool) (R:W->W->bool) (w:W) (x:W) <=>
+     ((R w x) /\ ~((w IN W) /\ (w  = x)))`;;
+
+let IRREFL_THEN_EQ = prove
+(`!(W:W->bool) (R:W->W->bool). IRREFLEXIVE W R ==> R = R_MIN W R`,
+  REWRITE_TAC[IRREFLEXIVE] THEN INTRO_TAC "!W R; irr" THEN
+   REWRITE_TAC[FUN_EQ_THM; R_MIN_DEF; R_PLUS_DEF] THEN
+   ASM_MESON_TAC[]);;
+
+let REFL_THEN_EQ = prove
+(`!(W:W->bool) (R:W->W->bool). REFLEXIVE W R ==> R = R_PLUS W (R_MIN W R)`,
+  REWRITE_TAC[REFLEXIVE] THEN INTRO_TAC "!W R; ref" THEN
+   REWRITE_TAC[FUN_EQ_THM; R_MIN_DEF; R_PLUS_DEF] THEN
+   ASM_MESON_TAC[]);;
+
+let ITF_IMP_R_PLUS_RATF = prove
+ (`!W:W->bool R. (W,R) IN ITF ==> (W,R_PLUS W R) IN RATF`,
+  REPEAT GEN_TAC THEN
+  REWRITE_TAC[IN_ITF; IN_RATF; IN_FINITE_FRAME] THEN
+  INTRO_TAC "(non_empty rel FINITE) IRR TRANS" THEN
+  ASM_REWRITE_TAC[] THEN
+  REPEAT CONJ_TAC THENL
+    [ASM_MESON_TAC[R_PLUS_DEF];
+     MESON_TAC[REFLEXIVE; R_PLUS_DEF];
+     HYP_TAC "TRANS" (REWRITE_RULE[TRANSITIVE]) THEN
+      REWRITE_TAC[TRANSITIVE; R_PLUS_DEF] THEN
+      ASM_MESON_TAC[];
+     HYP_TAC "IRR" (REWRITE_RULE[IRREFLEXIVE]) THEN
+     HYP_TAC "TRANS" (REWRITE_RULE[TRANSITIVE]) THEN
+     ASM_REWRITE_TAC[ANTISYMMETRIC; R_PLUS_DEF] THEN
+     ASM_MESON_TAC[]]);;
+
+let GRZ_TRANSL_LEMMA = prove
+  (`!p W R V w. (W:W->bool,R) IN ITF /\ w IN W ==>
+           (holds (W,R) V (TRANSL p) w <=> holds (W,R_PLUS W R) V p w)`,
+   FORM_INDUCT_TAC THENL
+   [REWRITE_TAC[TRANSL; holds];
+    REWRITE_TAC[TRANSL; holds];
+    REWRITE_TAC[TRANSL; holds];
+    ASM_REWRITE_TAC[TRANSL; holds] THEN ASM_MESON_TAC[];
+    ASM_REWRITE_TAC[TRANSL; holds] THEN ASM_MESON_TAC[];
+    ASM_REWRITE_TAC[TRANSL; holds] THEN ASM_MESON_TAC[];
+    ASM_REWRITE_TAC[TRANSL; holds] THEN ASM_MESON_TAC[];
+    ASM_REWRITE_TAC[TRANSL; holds] THEN ASM_MESON_TAC[];
+    INTRO_TAC "!W R V w; ITF w" THEN
+     REWRITE_TAC[TRANSL; dotbox_DEF; holds] THEN
+     MATCH_MP_TAC EQ_TRANS THEN
+     EXISTS_TAC
+      `!w'.  w' IN (W:W->bool) /\ R_PLUS W R w w'
+           ==> holds (W,R) V (TRANSL p) w'` THEN
+     ASM_MESON_TAC[R_PLUS_DEF]]);;
+
+let RATF_TRANSL = prove
+  (`!p. RATF:(form list->bool)#(form list->form list->bool)->bool |= p
+       <=> [GL_AX . {} |~ TRANSL (p)]`,
+  ONCE_REWRITE_TAC [TAUT `(P <=> Q) <=> (~P <=> ~Q)`] THEN
+   REWRITE_TAC[valid; holds_in; FORALL_PAIR_THM; NOT_FORALL_THM; NOT_IMP] THEN
+   GEN_TAC THEN EQ_TAC THENL
+   [REWRITE_TAC[IN_RATF; IN_FINITE_FRAME;
+                TRANSITIVE; ANTISYMMETRIC; REFLEXIVE] THEN
+    INTRO_TAC "@W R. ((non_empty rel FINITE) REFL TRANS ANTI) (@V w. IN not)" THEN
+    MP_TAC (INST_TYPE [`:form list`,`:W`] GL_ITF_VALID) THEN
+    INTRO_TAC "p" THEN
+    HYP_TAC "p" (ONCE_REWRITE_RULE[GSYM CONTRAPOS_THM]) THEN
+    FIRST_X_ASSUM MATCH_MP_TAC THEN
+    REWRITE_TAC[valid; holds_in; FORALL_PAIR_THM; NOT_FORALL_THM; NOT_IMP] THEN
+    EXISTS_TAC `W:form list->bool` THEN
+    EXISTS_TAC `R_MIN (W: form list->bool) (R:form list->form list->bool)` THEN
+    ASM_REWRITE_TAC[IN_ITF; IN_FINITE_FRAME] THEN REPEAT CONJ_TAC THENL
+    [ASM_MESON_TAC[R_MIN_DEF];
+     ASM_MESON_TAC[R_MIN_DEF; IRREFLEXIVE];
+     REWRITE_TAC[TRANSITIVE; R_MIN_DEF] THEN ASM_MESON_TAC[];
+     EXISTS_TAC `V:(char)list->(form)list->bool` THEN
+      EXISTS_TAC `w:form list` THEN ASM_REWRITE_TAC[] THEN
+      CLAIM_TAC "R_MIN_IN_ITF" `(W:form list->bool, R_MIN W R) IN ITF` THENL
+      [ASM_REWRITE_TAC[IN_ITF; IN_FINITE_FRAME; TRANSITIVE] THEN
+       REPEAT CONJ_TAC THENL
+       [ASM_MESON_TAC[R_MIN_DEF];
+        ASM_MESON_TAC[IRREFLEXIVE; R_MIN_DEF];
+        ASM_REWRITE_TAC[R_MIN_DEF] THEN  ASM_MESON_TAC[]]; ALL_TAC] THEN
+      MP_TAC (SPECL[`p:form`;
+                     `W:form list->bool`;
+                     `R_MIN W (R:form list -> form list ->bool)`;
+                     `V:char list->form list->bool`;
+                     `w:form list`] (INST_TYPE [`:form list`,`:W`] GRZ_TRANSL_LEMMA)) THEN
+      ASM_REWRITE_TAC[TAUT `(A=> (B <=>C)) => D <=> A=> (B<=>C) => D`] THEN
+      DISCH_TAC THEN ASM_REWRITE_TAC[] THEN
+      CLAIM_TAC "R_EQ" `R_PLUS W (R_MIN W R) = (R:form list->form list->bool)` THENL
+      [MATCH_MP_TAC (GSYM REFL_THEN_EQ) THEN
+       ASM_REWRITE_TAC[REFLEXIVE] THEN
+       ASM_REWRITE_TAC[]; ASM_REWRITE_TAC[]]];
+    INTRO_TAC "not_proves" THEN
+    SUBGOAL_THEN `~(ITF:(form list->bool)#(form list->form list->bool)->bool
+                   |= TRANSL (p:form))` MP_TAC THENL
+    [ASM_MESON_TAC[CONTRAPOS_THM; GL_COMPLETENESS_THM]; ALL_TAC] THEN
+    REWRITE_TAC[valid; holds_in; FORALL_PAIR_THM; NOT_FORALL_THM; NOT_IMP] THEN
+    INTRO_TAC "@W R. ITF (@V w. IN not)" THEN
+    EXISTS_TAC `W:form list->bool` THEN
+    EXISTS_TAC `R_PLUS (W:form list ->bool) (R:form list->form list ->bool)` THEN
+    CONJ_TAC THENL
+    [ASM_MESON_TAC[ITF_IMP_R_PLUS_RATF];
+     EXISTS_TAC `V:(char)list->(form)list->bool` THEN
+      EXISTS_TAC `w:form list` THEN
+      ASM_REWRITE_TAC[] THEN
+      CLAIM_TAC "R_IN_ITF"
+                `(W:form list->bool, R:form list->form list->bool) IN ITF` THENL
+      [ASM_REWRITE_TAC[IN_ITF; IN_FINITE_FRAME]; ALL_TAC] THEN
+      ASM_MESON_TAC[GRZ_TRANSL_LEMMA]]]);;
+
+let GRZ_TRANSL = prove
+  (`!p. [GRZ_AX . {} |~ p] <=> [GL_AX . {} |~ TRANSL (p)]`,
+    MESON_TAC[GRZ_ADEQ_THM; RATF_TRANSL]);;
+
+(* ------------------------------------------------------------------------- *)
+(* Decision procedure for the Grzegorczyk Logic (Grz) via translation to     *)
+(* Gödel-Löb provability Logic (GL).                                         *)
+(* ------------------------------------------------------------------------- *)
+
+let GRZ_TAC : tactic =
+  let vsubst_rplus = vsubst [`R_PLUS (W:num->bool) R`,`R:num->num->bool`] in
+  let tac =
+    GEN_REWRITE_TAC I [GRZ_TRANSL] THEN
+    CONV_TAC (RAND_CONV TRANSL_CONV) THEN
+    REWRITE_TAC[dotbox_DEF] THEN
+    GL_TAC in
+  (* Call tac and translate countermodel in case of failure *)
+  fun gl ->
+    try tac gl with Failure s ->
+      the_HOLMS_countermodel := vsubst_rplus !the_HOLMS_countermodel;
+      FAIL_TAC s gl;;
+
+holms_register_tactic `GRZ_AX` GRZ_TAC;;
+
+(* ------------------------------------------------------------------------- *)
+(* Tests and examples.                                                       *)
+(* ------------------------------------------------------------------------- *)
+
+(* Example: Box (Box (a --> Box a) --> a) --> a *)
+let tm = `[GRZ_AX . {} |~ Box (Box (Atom a --> Box Atom a) --> Atom a)
+                          --> Atom a]`;;
+time HOLMS_RULE tm;;
+g tm;;
+time e HOLMS_TAC;;
+top_thm();;
+
+(* Example: Same as before, but with metavariables. *)
+(* let tm = `[GRZ_AX . {} |~ Box (Box (a --> Box a) --> a) --> a]`;; *)
+(* time HOLMS_RULE tm;; *)
+
+(* Example: Box a --> a *)
+let tm = `[GRZ_AX . {} |~ Box Atom "a" --> Atom "a"]`;;
+time HOLMS_RULE tm;;
+
+(* ------------------------------------------------------------------------- *)
+(* Decision procedure.                                                       *)
+(* ------------------------------------------------------------------------- *)
+
+let GRZ_CONV : conv =
+  GEN_REWRITE_CONV I [GRZ_TRANSL] THENC
+  GEN_REWRITE_CONV (RAND_CONV o TOP_DEPTH_CONV)
+                   [TRANSL; diam_DEF; dotbox_DEF] THENC
+  GL_CONV THENC
+  REWRITE_CONV[];;
