grz_tests.ml
@@ -1,0 +1,69 @@
+(* ========================================================================= *)
+(* Tests for the Grzegorczyk Logic (Grz).                                    *)
+(*                                                                           *)
+(* (c) Copyright, Antonella Bilotta, Marco Maggesi,                          *)
+(*                Cosimo Perini Brogi 2025-26.                               *)
+(* ========================================================================= *)
+
+needs "HOLMS/grz.ml";;
+
+(* ------------------------------------------------------------------------- *)
+(* Basic usage examples.                                                     *)
+(* ------------------------------------------------------------------------- *)
+
+HOLMS_RULE `[GRZ_AX . {}
+             |~ Box (Box (Atom "p" --> Box Atom "p") --> Atom "p")
+                --> Atom "p"]`;;
+
+HOLMS_BUILD_COUNTERMODEL
+  `[GRZ_AX . {} |~  Box(Box Atom "p" --> Atom "p") --> Box Atom "p"]`;;
+
+GRZ_CONV `[GRZ_AX . {}
+           |~ Box (Box (Atom "p" --> Box Atom "p") --> Atom "p")
+              --> Atom "p"]`;;
+
+GRZ_CONV `[GRZ_AX . {} |~  Box(Box Atom "p" --> Atom "p") --> Box Atom "p"]`;;
+
+(* ------------------------------------------------------------------------- *)
+(* Tests, examples.                                                          *)
+(* ------------------------------------------------------------------------- *)
+
+let pnames = explode "abpqr";;
+let pvars = map (fun s -> mk_var(s,form_ty)) pnames
+and patoms = map (mk_modal_atom o mk_string) pnames;;
+let ipatoms = zip patoms pvars;;
+let [atm;btm;ptm;qtm;rtm] = pvars;;
+let [a_atom;b_atom;p_atom;q_atom;r_atom] = patoms;;
+
+(* ------------------------------------------------------------------------- *)
+(* GZR tests.                                                                *)
+(* ------------------------------------------------------------------------- *)
+
+let mk_grz_proves =
+  let grzv_tm = `[GRZ_AX . {} |~ p]` in
+  fun tm -> let tm' = vsubst ipatoms tm in
+            vsubst [tm',ptm] grzv_tm;;
+
+let test_grz_proves = check_conv_true GRZ_CONV o mk_grz_proves;;
+let test_grz_disproves = check_conv_false GRZ_CONV o mk_grz_proves;;
+
+(* Proves. *)
+test_grz_proves `Box (Box (p --> Box p) --> p) --> p`;;
+test_grz_proves `Box p --> p`;;
+test_grz_proves `Box Box p --> Box p`;;
+test_grz_proves `Box p --> Diam p`;;
+test_grz_proves `Box (p --> q) --> (Box p --> q)`;;
+test_grz_proves `Box (p --> Box q) --> (p --> q)`;;
+test_grz_proves `Diam Box p --> Diam p`;;
+test_grz_proves `((a --> Box b) --> Box b) && ((Not a --> Box b) --> Box b) --> Box b`;;
+test_grz_proves `Box(Box(a --> Box a) --> Box a) --> Box a`;;
+test_grz_proves `(Not p --> Not q) --> (q --> p)`;;
+
+(* Disproves. *)
+test_grz_disproves `Box(Box a --> a) --> Box a`;;
+test_grz_disproves `Diam a --> Box Diam a`;;
+test_grz_disproves `Box(Box a --> b) && Box(Box b --> a)`;;
+test_grz_disproves `a --> Diam Box a`;;
+test_grz_disproves `Diam Box a --> Box Diam a`;;
+test_grz_disproves `p || (Not p && Box(p --> Box p))`;;
+test_grz_disproves `Box Diam a --> Box b`;;
