schematic.ml
@@ -1,0 +1,49 @@
+(* ========================================================================= *)
+(* Esperimento: Cambiare atomi con metavariabili e viceversa usando SUBST.   *)
+(* ========================================================================= *)
+
+(* ------------------------------------------------------------------------- *)
+(* Lemmata.                                                                  *)
+(* ------------------------------------------------------------------------- *)
+
+let SUBST_IMP_ALT = prove
+ (`!S H p. [S . H |~ p]
+           ==> !f. (!q. q IN S ==> SUBST f q IN S)
+                   ==> [S . IMAGE (SUBST f) H |~ SUBST f p]`,
+  MESON_TAC[SUBST_IMP]);;
+
+let FORALL_IN_GL_AX = prove
+ (`!P. (!p. p IN GL_AX ==> P p) <=> (!p. P (LOB_SCHEMA p))`,
+  REWRITE_TAC[GL_AX; FORALL_IN_GSPEC; IN_UNIV]);;
+
+let SUBST_LOB_SCHEMA = prove
+ (`!f p. SUBST f (LOB_SCHEMA p) = LOB_SCHEMA (SUBST f p)`,
+  REWRITE_TAC[SUBST; LOB_SCHEMA_DEF]);;
+
+let GL_SCHEMATIC = prove
+ (`!p. p IN GL_AX ==> SUBST f p IN GL_AX`,
+  REWRITE_TAC[FORALL_IN_GL_AX; SUBST_LOB_SCHEMA] THEN
+  REWRITE_TAC[GL_AX] THEN SET_TAC[]);;
+
+(* ------------------------------------------------------------------------- *)
+(* Esempio: p --> q                                                          *)
+(* ------------------------------------------------------------------------- *)
+
+g `[GL_AX . {} |~ Atom "p" --> Atom "q"] <=>
+   (!p q. [GL_AX . {} |~ p --> q])`;;
+e (SUBGOAL_THEN
+    `[GL_AX . {} |~ Atom "p" --> Atom "q"]
+     ==> (!p q. [GL_AX . {} |~ p --> q])`
+    (fun th -> MESON_TAC[th]));;
+e (INTRO_TAC "hp; !p q");;
+e (POP_ASSUM (MP_TAC o MATCH_MP SUBST_IMP_ALT));;
+e (REWRITE_TAC[IMAGE_CLAUSES; GL_SCHEMATIC]);;
+e (DISCH_THEN (MP_TAC o SPEC `\s. if s = "p" then p else q:form`));;
+e (REWRITE_TAC[SUBST; CONS_11; injectivity "char"]);;
+top_thm();;
+
+let tm = `[GL_AX . {} |~ Atom "p" --> Atom "q"]`;;
+let atoms = find_terms is_modal_atom tm;;
+let ctx = map (fun a -> a,genvar `:form`) atoms;;
+let swap(x,y) = y,x;;
+subst (map swap ctx) tm;;
